Core_Erlang_Helpers.v
@@ -55,18 +55,18 @@ end.
 (** Pattern matching success checker *)
 Fixpoint match_value_to_pattern (e : Value) (p : Pattern) : bool :=
 match p with
-| PEmptyList => 
+| PNil => 
    match e with
-   | VEmptyList => true
+   | VNil => true
    | _ => false
    end
 | PVar v => true (* every e matches to a pattern variable *)
-| PLiteral l => match e with
-  | VLiteral l' => match_literals l l'
+| PLit l => match e with
+  | VLit l' => match_literals l l'
   | _ => false
   end
-| PList hd tl => match e with
-  | VList hd' tl' => (match_value_to_pattern hd' hd) && (match_value_to_pattern tl' tl)
+| PCons hd tl => match e with
+  | VCons hd' tl' => (match_value_to_pattern hd' hd) && (match_value_to_pattern tl' tl)
   | _ => false
   end
 | PTuple l => match e with
@@ -84,22 +84,22 @@ end
 .
 
 (** Examples *)
-Compute match_value_to_pattern (VClosure [] [] 0 [] ErrorExp) (PVar "X"%string).
-Compute match_value_to_pattern (VLiteral (Atom "a"%string)) (PVar "X"%string).
-Compute match_value_to_pattern (VLiteral (Atom "a"%string)) (PLiteral (Atom "a"%string)).
-Compute match_value_to_pattern (VLiteral (Atom "a"%string)) (PEmptyTuple).
-Compute match_value_to_pattern (VTuple [VLiteral (Atom "a"%string) ; VLiteral (Integer 1)]) 
+Compute match_value_to_pattern (VClos [] [] 0 [] ErrorExp) (PVar "X"%string).
+Compute match_value_to_pattern (VLit (Atom "a"%string)) (PVar "X"%string).
+Compute match_value_to_pattern (VLit (Atom "a"%string)) (PLit (Atom "a"%string)).
+Compute match_value_to_pattern (VLit (Atom "a"%string)) (PEmptyTuple).
+Compute match_value_to_pattern (VTuple [VLit (Atom "a"%string) ; VLit (Integer 1)]) 
                                (PVar "X"%string).
-Compute match_value_to_pattern (VTuple [VLiteral (Atom "a"%string) ; VLiteral (Integer 1)]) 
-                               (PTuple [PVar "X"%string ; PLiteral (Integer 1)]).
+Compute match_value_to_pattern (VTuple [VLit (Atom "a"%string) ; VLit (Integer 1)]) 
+                               (PTuple [PVar "X"%string ; PLit (Integer 1)]).
 
 (** Used variables in a pattern *)
 Fixpoint variable_occurances (p : Pattern) : list Var :=
 match p with
- | PEmptyList => []
+ | PNil => []
  | PVar v => [v]
- | PLiteral l => []
- | PList hd tl => variable_occurances hd ++ variable_occurances tl
+ | PLit l => []
+ | PCons hd tl => variable_occurances hd ++ variable_occurances tl
  | PTuple l => (fix variable_occurances_list l :=
                    match l with
                    | [] => []
@@ -110,10 +110,10 @@ end.
 (** Used variables in a pattern, but now with sets *)
 Fixpoint variable_occurances_set (p : Pattern) : set Var :=
 match p with
- | PEmptyList => []
+ | PNil => []
  | PVar v => [v]
- | PLiteral l => []
- | PList hd tl => set_union string_dec (variable_occurances_set hd)
+ | PLit l => []
+ | PCons hd tl => set_union string_dec (variable_occurances_set hd)
                                        (variable_occurances_set tl)
  | PTuple l => (fix variable_occurances_set_list t :=
                     match t with
@@ -129,17 +129,17 @@ end.
     Should be used together with match_value_to_pattern *)
 Fixpoint match_value_bind_pattern (e : Value) (p : Pattern) : list (Var * Value) :=
 match p with
-| PEmptyList => match e with
-                | VEmptyList => []
+| PNil => match e with
+                | VNil => []
                 | _ => [] (** error *)
                 end
 | PVar v => [(v, e)] (** every e matches to a pattern variable *)
-| PLiteral l => match e with
-  | VLiteral l' => if match_literals l l' then [] else [] (* Error *)
+| PLit l => match e with
+  | VLit l' => if match_literals l l' then [] else [] (* Error *)
   | _ => [] (** error *)
   end
-| PList hd tl => match e with
-  | VList hd' tl' => (match_value_bind_pattern hd' hd) ++ (match_value_bind_pattern tl' tl)
+| PCons hd tl => match e with
+  | VCons hd' tl' => (match_value_bind_pattern hd' hd) ++ (match_value_bind_pattern tl' tl)
   | _ => [] (** error *)
   end
 | PTuple pl => match e with
@@ -162,17 +162,17 @@ end
 .
 
 (** Examples *)
-Compute match_value_bind_pattern (VClosure [] [] 0 [] ErrorExp) (PVar "X"%string).
-Compute match_value_bind_pattern (VLiteral (Atom "a"%string)) (PVar "X"%string).
-Compute match_value_bind_pattern (VLiteral (Atom "a"%string)) (PLiteral (Atom "alma"%string)).
-Compute match_value_bind_pattern (VLiteral (Atom "a"%string)) (PEmptyTuple).
-Compute match_value_bind_pattern (VTuple [VLiteral (Atom "a"%string) ; VLiteral (Integer 1)]) 
+Compute match_value_bind_pattern (VClos [] [] 0 [] ErrorExp) (PVar "X"%string).
+Compute match_value_bind_pattern (VLit (Atom "a"%string)) (PVar "X"%string).
+Compute match_value_bind_pattern (VLit (Atom "a"%string)) (PLit (Atom "alma"%string)).
+Compute match_value_bind_pattern (VLit (Atom "a"%string)) (PEmptyTuple).
+Compute match_value_bind_pattern (VTuple [VLit (Atom "a"%string) ; VLit (Integer 1)]) 
                                  (PVar "X"%string).
-Compute match_value_to_pattern (VTuple [VLiteral (Atom "a"%string) ; 
-                                        VLiteral (Integer 1); VLiteral (Integer 2)]) 
+Compute match_value_to_pattern (VTuple [VLit (Atom "a"%string) ; 
+                                        VLit (Integer 1); VLit (Integer 2)]) 
                                (PTuple [PVar "X"%string ; PVar "Y"%string]).
-Compute match_value_bind_pattern (VTuple [VLiteral (Atom "a"%string) ; VLiteral (Integer 1); 
-                                          VLiteral (Integer 2)]) 
+Compute match_value_bind_pattern (VTuple [VLit (Atom "a"%string) ; VLit (Integer 1); 
+                                          VLit (Integer 2)]) 
                                  (PTuple [PVar "X"%string ; PVar "Y"%string]).
 
 (** From the list of patterns, guards and bodies, this function 
@@ -208,18 +208,18 @@ Compute variable_occurances_set (PTuple [PVar "X"%string ; PVar "X"%string]).
 (** Get the used variables of an expression *)
 Fixpoint variables (e : Expression) : list Var :=
 match e with
-| EEmptyList => []
-| ELiteral l => []
+| ENil => []
+| ELit l => []
 | EVar     v => [v]
 | EFunId   f => []
 | EFun  vl e => variables e
-| EList hd tl => variables hd ++ variables tl
+| ECons hd tl => variables hd ++ variables tl
 | ETuple l => flat_map variables l
 | ECall  f l => flat_map variables l
-| EApply exp l => flat_map variables l ++ variables exp
+| EApp exp l => flat_map variables l ++ variables exp
 | ECase  e ps gs bs => variables e ++ flat_map variables gs ++ flat_map variables bs
 | ELet s el e => flat_map variables el ++ variables e
-| ELetrec fn vs bs e => variables e (** Extesion needed maybe *)
+| ELetRec fn vs bs e => variables e (** Extesion needed maybe *)
 | EMap  kl vl => flat_map variables kl ++ flat_map variables vl
 | ETry e e1 e2 v vex1 vex2 vex3 => [v; vex1; vex2; vex3] ++ 
                                    variables e ++ variables e1 ++ variables e2
@@ -252,8 +252,8 @@ match kl, vl with
 | _, _ => ([], [])
 end.
 
-Compute make_value_map [VLiteral (Integer 5); VLiteral (Integer 5); VLiteral (Atom ""%string)] 
-                       [VLiteral (Integer 5); VLiteral (Integer 7); VLiteral (Atom ""%string)].
+Compute make_value_map [VLit (Integer 5); VLit (Integer 5); VLit (Atom ""%string)] 
+                       [VLit (Integer 5); VLit (Integer 7); VLit (Atom ""%string)].
 
 Definition nth_id (ids : list nat) (def i : nat) :=
 match i with
