Core_Erlang_Side_Effect_Tests.v
@@ -15,23 +15,23 @@ Import Core_Erlang_Semantics.
 
 
 Example tuple_eff :
-  |[], ETuple [ECall "fwrite"%string [ELiteral (Atom "a"%string)];
-               ECall "fwrite"%string [ELiteral (Atom "b"%string)];
-               ECall "fread"%string [ELiteral (Atom ""%string) ; ELiteral (Atom "c"%string)]], []|
+  |[], ETuple [ECall "fwrite"%string [ELit (Atom "a"%string)];
+               ECall "fwrite"%string [ELit (Atom "b"%string)];
+               ECall "fread"%string [ELit (Atom ""%string) ; ELit (Atom "c"%string)]], []|
 -e>
-  |inl (VTuple [ok;ok; VTuple [ok; VLiteral (Atom "c"%string)]]), 
-   [(Output, [VLiteral (Atom "a"%string)]); (Output, [VLiteral (Atom "b"%string)]);
-    (Input, [VLiteral (Atom ""%string); VLiteral (Atom "c"%string)])]|.
+  |inl (VTuple [ok;ok; VTuple [ok; VLit (Atom "c"%string)]]), 
+   [(Output, [VLit (Atom "a"%string)]); (Output, [VLit (Atom "b"%string)]);
+    (Input, [VLit (Atom ""%string); VLit (Atom "c"%string)])]|.
 Proof.
-  apply eval_tuple with (eff := [[(Output, [VLiteral (Atom "a"%string)])]; 
-                                 [(Output, [VLiteral (Atom "b"%string)])]; 
-                                 [(Input, [VLiteral (Atom ""%string); 
-                                           VLiteral (Atom "c"%string)])]]).
+  apply eval_tuple with (eff := [[(Output, [VLit (Atom "a"%string)])]; 
+                                 [(Output, [VLit (Atom "b"%string)])]; 
+                                 [(Input, [VLit (Atom ""%string); 
+                                           VLit (Atom "c"%string)])]]).
   * reflexivity.
   * simpl. reflexivity.
   * intros. inversion H.
-    - subst. simpl. apply eval_call with (vals := [VLiteral (Atom ""%string); 
-                                                   VLiteral (Atom "c"%string)])
+    - subst. simpl. apply eval_call with (vals := [VLit (Atom ""%string); 
+                                                   VLit (Atom "c"%string)])
                                          (eff := [ []; [] ]).
       + reflexivity.
       + reflexivity.
@@ -41,7 +41,7 @@ Proof.
           -- apply eval_lit.
           -- inversion H4.
       + unfold concatn. simpl. reflexivity.
-    - inversion H1. simpl. apply eval_call with (vals := [VLiteral (Atom "b"%string)])
+    - inversion H1. simpl. apply eval_call with (vals := [VLit (Atom "b"%string)])
                                                 (eff := [[]]).
       + reflexivity.
       + reflexivity.
@@ -49,7 +49,7 @@ Proof.
         ** apply eval_lit.
         ** inversion H5.
       + simpl. reflexivity.
-      + inversion H3. simpl. apply eval_call with (vals := [VLiteral (Atom "a"%string)])
+      + inversion H3. simpl. apply eval_call with (vals := [VLit (Atom "a"%string)])
                                                   (eff := [[]]).
         ** reflexivity.
         ** reflexivity.
@@ -62,20 +62,20 @@ Proof.
 Qed.
 
 Example list_eff :
-  |[], EList (ECall "fwrite"%string [ELiteral (Atom "a")])
-             (EList (ECall "fwrite"%string [ELiteral (Atom "b")]) EEmptyList), []|
+  |[], ECons (ECall "fwrite"%string [ELit (Atom "a")])
+             (ECons (ECall "fwrite"%string [ELit (Atom "b")]) ENil), []|
 -e> 
-  |inl (VList ok (VList ok VEmptyList)), 
-   [(Output, [VLiteral (Atom "b")]); (Output, [VLiteral (Atom "a")])]|.
+  |inl (VCons ok (VCons ok VNil)), 
+   [(Output, [VLit (Atom "b")]); (Output, [VLit (Atom "a")])]|.
 Proof.
-  eapply eval_list with (eff2 := [(Output, [VLiteral (Atom "b")])]).
+  eapply eval_list with (eff2 := [(Output, [VLit (Atom "b")])]).
   * simpl. reflexivity.
   * simpl. eapply eval_list with (eff2 := []).
     - simpl. reflexivity.
     - apply eval_emptylist.
-    - eapply eval_call with (vals := [VLiteral (Atom "b")]) (eff := [[]]); auto.
+    - eapply eval_call with (vals := [VLit (Atom "b")]) (eff := [[]]); auto.
       + intros. inversion H. 2: inversion H1. apply eval_lit.
-  * simpl. eapply eval_call with (vals := [VLiteral (Atom "a")]) (eff := [[]]).
+  * simpl. eapply eval_call with (vals := [VLit (Atom "a")]) (eff := [[]]).
     - reflexivity.
     - reflexivity.
     - intros. inversion H. 2: inversion H1. apply eval_lit.
@@ -83,19 +83,19 @@ Proof.
 Qed.
 
 Example case_eff : 
-  |[], ECase (ECall "fwrite"%string [ELiteral (Atom "a")])
-           [PVar "X"%string; PLiteral (Integer 5); PVar "Y"%string]
-           [ELiteral (Atom "false"); ELiteral (Atom "true"); 
-            ELiteral (Atom "true")]
-           [(ECall "fwrite"%string [ELiteral (Atom "b")]); 
-            ELiteral (Integer 2); 
-            (ECall "fwrite"%string [ELiteral (Atom "c")])]
+  |[], ECase (ECall "fwrite"%string [ELit (Atom "a")])
+           [PVar "X"%string; PLit (Integer 5); PVar "Y"%string]
+           [ELit (Atom "false"); ELit (Atom "true"); 
+            ELit (Atom "true")]
+           [(ECall "fwrite"%string [ELit (Atom "b")]); 
+            ELit (Integer 2); 
+            (ECall "fwrite"%string [ELit (Atom "c")])]
   , []|
 -e>
-  |inl ok, [(Output, [VLiteral (Atom "a")]); (Output, [VLiteral (Atom "c")])]|.
+  |inl ok, [(Output, [VLit (Atom "a")]); (Output, [VLit (Atom "c")])]|.
 Proof.
   eapply eval_case with (i := 2); auto.
-  * eapply eval_call with (vals := [VLiteral (Atom "a")]) (eff :=[[]]); auto.
+  * eapply eval_call with (vals := [VLit (Atom "a")]) (eff :=[[]]); auto.
     - intros. inversion H. 2: inversion H1. apply eval_lit.
     - simpl. reflexivity.
   * simpl. reflexivity.
@@ -104,116 +104,116 @@ Proof.
     - subst. inversion H0. apply eval_lit.
   * simpl. reflexivity.
   * simpl. apply eval_lit.
-  * simpl. eapply eval_call with (vals := [VLiteral (Atom "c")]) (eff := [[]]); auto.
+  * simpl. eapply eval_call with (vals := [VLit (Atom "c")]) (eff := [[]]); auto.
     - intros. inversion H. 2: inversion H1. unfold concatn. simpl. apply eval_lit.
 Qed.
 
 Example call_eff :
-  |[], ECall "fwrite"%string [ECall "fwrite"%string [ELiteral (Atom "a")]], []|
+  |[], ECall "fwrite"%string [ECall "fwrite"%string [ELit (Atom "a")]], []|
 -e>
-  |inl ok, [(Output, [VLiteral (Atom "a")]); (Output, [ok])]|.
+  |inl ok, [(Output, [VLit (Atom "a")]); (Output, [ok])]|.
 Proof.
-  eapply eval_call with (vals := [ok]) (eff := [[(Output, [VLiteral (Atom "a")])]]); auto.
+  eapply eval_call with (vals := [ok]) (eff := [[(Output, [VLit (Atom "a")])]]); auto.
   * intros. inversion H. 2: inversion H1. simpl. 
-    eapply eval_call with (vals := [VLiteral (Atom "a")]) (eff := [[]]); auto.
+    eapply eval_call with (vals := [VLit (Atom "a")]) (eff := [[]]); auto.
     - intros. inversion H0. 2: inversion H3. unfold concatn. simpl. apply eval_lit.
 Qed.
 
 Example apply_eff : 
-  |[(inl "Y"%string, VClosure [] [] 0 ["Z"%string] (ECall "fwrite"%string [ELiteral (Atom "c")]))], 
-    EApply (ELet ["X"%string] [ECall "fwrite"%string [ELiteral (Atom "a")]] 
+  |[(inl "Y"%string, VClos [] [] 0 ["Z"%string] (ECall "fwrite"%string [ELit (Atom "c")]))], 
+    EApp (ELet ["X"%string] [ECall "fwrite"%string [ELit (Atom "a")]] 
              (EVar "Y"%string))
-           [ECall "fwrite" [ELiteral (Atom "b")] ], []|
+           [ECall "fwrite" [ELit (Atom "b")] ], []|
 -e>
   |inl ok, 
-   [(Output, [VLiteral (Atom "a")]);
-    (Output, [VLiteral (Atom "b")]);
-    (Output, [VLiteral (Atom "c")])]|.
+   [(Output, [VLit (Atom "a")]);
+    (Output, [VLit (Atom "b")]);
+    (Output, [VLit (Atom "c")])]|.
 Proof.
-  eapply eval_apply with (vals := [ok]) (eff := [[(Output, [VLiteral (Atom "b")])]]) 
+  eapply eval_apply with (vals := [ok]) (eff := [[(Output, [VLit (Atom "b")])]]) 
                          (ref := []) (ext := []) (var_list := ["Z"%string]) (n := 0)
-                         (body := ECall "fwrite"%string [ELiteral (Atom "c")]).
+                         (body := ECall "fwrite"%string [ELit (Atom "c")]).
   * reflexivity.
-  * eapply eval_let with (vals := [ok]) (eff := [[(Output, [VLiteral (Atom "a")])]]).
+  * eapply eval_let with (vals := [ok]) (eff := [[(Output, [VLit (Atom "a")])]]).
     - reflexivity.
     - reflexivity.
     - intros. inversion H. 2: inversion H1. 
-      eapply eval_call with (vals := [VLiteral (Atom "a")]) (eff := [[]]); auto.
+      eapply eval_call with (vals := [VLit (Atom "a")]) (eff := [[]]); auto.
       + intros. inversion H0. 2: inversion H3. apply eval_lit.
     - unfold concatn. simpl. reflexivity.
     - simpl. apply eval_var.
   * reflexivity.
   * reflexivity.
   * intros. inversion H. 2: inversion H1. unfold concatn. simpl. 
-    apply eval_call with (vals := [VLiteral (Atom "b")]) (eff := [[]]); auto.
+    apply eval_call with (vals := [VLit (Atom "b")]) (eff := [[]]); auto.
     - intros. inversion H0. 2: inversion H3. simpl. apply eval_lit.
   * unfold concatn. simpl. reflexivity.
-  * simpl. eapply eval_call with (vals := [VLiteral (Atom "c")]) (eff := [[]]); auto.
+  * simpl. eapply eval_call with (vals := [VLit (Atom "c")]) (eff := [[]]); auto.
     - intros. inversion H. 2: inversion H1. apply eval_lit.
 Qed.
 
 Example let_eff : 
-  |[], ELet ["X"%string; "Y"%string] [ECall "fwrite"%string [ELiteral (Atom "a")]; 
-                                      EFun [] (ECall "fwrite"%string [ELiteral (Atom "b")])]
-          (EApply (EVar "Y"%string) []), []|
+  |[], ELet ["X"%string; "Y"%string] [ECall "fwrite"%string [ELit (Atom "a")]; 
+                                      EFun [] (ECall "fwrite"%string [ELit (Atom "b")])]
+          (EApp (EVar "Y"%string) []), []|
 -e>
-  |inl ok, [(Output, [VLiteral (Atom "a")]); (Output, [VLiteral (Atom "b")])]|.
+  |inl ok, [(Output, [VLit (Atom "a")]); (Output, [VLit (Atom "b")])]|.
 Proof.
   eapply eval_let with (vals := [ok;
-                                 VClosure [] [] 0 [] (ECall "fwrite"%string [ELiteral (Atom "b")])])
-                       (eff := [[(Output, [VLiteral (Atom "a")])]; []]); auto.
+                                 VClos [] [] 0 [] (ECall "fwrite"%string [ELit (Atom "b")])])
+                       (eff := [[(Output, [VLit (Atom "a")])]; []]); auto.
   * intros. inversion H. 2: inversion H1. 3: inversion H3.
     - simpl. apply eval_fun.
-    - simpl. eapply eval_call with (vals := [VLiteral (Atom "a")]) (eff := [[]]); auto.
+    - simpl. eapply eval_call with (vals := [VLit (Atom "a")]) (eff := [[]]); auto.
       + intros. inversion H2. 2: inversion H5. apply eval_lit. 
   * unfold concatn. simpl. reflexivity.
   * eapply eval_apply with (vals := []) (var_list := []) 
                            (ref := []) (ext := []) (n := 0)
-                           (body := ECall "fwrite"%string [ELiteral (Atom "b")]) 
+                           (body := ECall "fwrite"%string [ELit (Atom "b")]) 
                            (eff := []); auto.
     - simpl. apply eval_var.
     - intros. inversion H.
     - simpl. reflexivity.
-    - simpl. eapply eval_call with (vals := [VLiteral (Atom "b")]) (eff := [[]]); auto.
+    - simpl. eapply eval_call with (vals := [VLit (Atom "b")]) (eff := [[]]); auto.
       + intros. inversion H. 2: inversion H1. apply eval_lit.
 Qed.
 
 Example letrec_eff : 
-  |[], ELetrec [("f1"%string, 0)] [[]] 
-              [ECall "fwrite"%string [ELiteral (Atom "a")]]
-        (EApply (EFunId ("f1"%string, 0)) []), []|
+  |[], ELetRec [("f1"%string, 0)] [[]] 
+              [ECall "fwrite"%string [ELit (Atom "a")]]
+        (EApp (EFunId ("f1"%string, 0)) []), []|
 -e>
-  |inl ok, [(Output, [VLiteral (Atom "a")])]|.
+  |inl ok, [(Output, [VLit (Atom "a")])]|.
 Proof.
   eapply eval_letrec; auto.
   2 : reflexivity.
   * simpl. eapply eval_apply with (vals := []) (eff := []) (ref := []) 
                                   (ext := [("f1"%string, 0, ([], ECall "fwrite" 
-                                                                 [ELiteral (Atom "a")]))]) 
+                                                                 [ELit (Atom "a")]))]) 
                                   (var_list := []) (n := 0)
-                                  (body := ECall "fwrite"%string [ELiteral (Atom "a")]); auto.
+                                  (body := ECall "fwrite"%string [ELit (Atom "a")]); auto.
     - apply eval_funid.
     - intros. inversion H.
     - simpl. reflexivity.
-    - simpl. apply eval_call with (vals := [VLiteral (Atom "a")]) (eff := [[]]); auto.
+    - simpl. apply eval_call with (vals := [VLit (Atom "a")]) (eff := [[]]); auto.
       + intros. inversion H. 2: inversion H1. apply eval_lit.
 Qed.
 
 Example map_eff : 
-  |[], EMap [ECall "fwrite"%string [ELiteral (Atom "a"%string)];
-             ECall "fwrite"%string [ELiteral (Atom "c"%string)]]
-            [ECall "fwrite"%string [ELiteral (Atom "b"%string)];
-             ELiteral (Integer 5)], []| 
+  |[], EMap [ECall "fwrite"%string [ELit (Atom "a"%string)];
+             ECall "fwrite"%string [ELit (Atom "c"%string)]]
+            [ECall "fwrite"%string [ELit (Atom "b"%string)];
+             ELit (Integer 5)], []| 
 -e> 
-  | inl (VMap [ok] [VLiteral (Integer 5)]),
-    [(Output, [VLiteral (Atom "a"%string)]);
-     (Output, [VLiteral (Atom "b"%string)]);
-     (Output, [VLiteral (Atom "c"%string)])]|.
+  | inl (VMap [ok] [VLit (Integer 5)]),
+    [(Output, [VLit (Atom "a"%string)]);
+     (Output, [VLit (Atom "b"%string)]);
+     (Output, [VLit (Atom "c"%string)])]|.
 Proof.
-  apply eval_map with (kvals := [ok; ok]) (vvals := [ok; VLiteral (Integer 5)])
-                      (eff := [[(Output, [VLiteral (Atom "a")])]; 
-                               [(Output, [VLiteral (Atom "b")])]; 
-                               [(Output, [VLiteral (Atom "c")])]; 
+  apply eval_map with (kvals := [ok; ok]) (vvals := [ok; VLit (Integer 5)])
+                      (eff := [[(Output, [VLit (Atom "a")])]; 
+                               [(Output, [VLit (Atom "b")])]; 
+                               [(Output, [VLit (Atom "c")])]; 
                                []]).
   * reflexivity.
   * reflexivity.
@@ -221,7 +221,7 @@ Proof.
   * reflexivity.
   * simpl. reflexivity.
   * unfold concatn. intros. inversion H.
-    - apply eval_call with (vals := [VLiteral (Atom "c")]) (eff := [[]]).
+    - apply eval_call with (vals := [VLit (Atom "c")]) (eff := [[]]).
       + reflexivity.
       + reflexivity.
       + intros. inversion H0.
@@ -229,7 +229,7 @@ Proof.
         ** inversion H3.
       + unfold concatn. simpl. reflexivity.
     - inversion H1.
-      + simpl. apply eval_call with (vals := [VLiteral (Atom "a")]) (eff := [[]]).
+      + simpl. apply eval_call with (vals := [VLit (Atom "a")]) (eff := [[]]).
         ** reflexivity.
         ** reflexivity.
         ** intros. inversion H2. 2: inversion H5. simpl. apply eval_lit.
@@ -238,7 +238,7 @@ Proof.
   * intros. inversion H.
     - simpl. apply eval_lit.
     - inversion H1.
-      + apply eval_call with (vals := [VLiteral (Atom "b")]) (eff := [[]]).
+      + apply eval_call with (vals := [VLit (Atom "b")]) (eff := [[]]).
         ** reflexivity.
         ** reflexivity.
         ** intros. inversion H2. 2: inversion H5. simpl. apply eval_lit.
