Core_Erlang_Tests.v
@@ -15,19 +15,19 @@ Import Core_Erlang_Side_Effects.
 
 (** This is an edless recursion *)
 Example eval_letrec1 : 
-  |[], 0, ELetrec [("x"%string, 1)] [["X"%string]] 
-         [EApply (EFunId ("x"%string, 1)) [EVar "X"%string]] 
-            (EApply (EFunId ("x"%string, 1)) [EEmptyTuple]), []|
+  |[], 0, ELetRec [("x"%string, 1)] [["X"%string]] 
+         [EApp (EFunId ("x"%string, 1)) [EVar "X"%string]] 
+            (EApp (EFunId ("x"%string, 1)) [EEmptyTuple]), []|
 -e> 
   |1, inl ErrorValue, []|.
 Proof.
   eapply eval_letrec; try (reflexivity).
   * simpl. eapply eval_apply with (vals := [VEmptyTuple]) 
-                                  (body := (EApply (EFunId ("x"%string, 1)) [EVar "X"%string])) (n := 0) (ids := [1])
+                                  (body := (EApp (EFunId ("x"%string, 1)) [EVar "X"%string])) (n := 0) (ids := [1])
                                   (var_list := ["X"%string]) 
                                   (ref := [])
                                   (ext := [(0, ("x"%string, 1), 
-                                        (["X"%string], EApply (EFunId ("x"%string, 1)) [EVar "X"%string]))]) 
+                                        (["X"%string], EApp (EFunId ("x"%string, 1)) [EVar "X"%string]))]) 
                                   (eff := [[]]); try (reflexivity).
     - unfold append_funs_to_env. simpl. eapply eval_funid.
     - intros. inversion H.
@@ -37,11 +37,11 @@ Proof.
       + inversion H1.
     - simpl. reflexivity.
     - eapply eval_apply with (vals := [VEmptyTuple]) 
-                             (body := (EApply (EFunId ("x"%string, 1)) [EVar "X"%string])) 
+                             (body := (EApp (EFunId ("x"%string, 1)) [EVar "X"%string])) 
                              (var_list := ["X"%string]) 
                              (ref := []) (ids := [1])
                              (ext := [(0, ("x"%string, 1),
-                                     (["X"%string], EApply (EFunId ("x"%string, 1)) [EVar "X"%string]))]) (n := 0)
+                                     (["X"%string], EApp (EFunId ("x"%string, 1)) [EVar "X"%string]))]) (n := 0)
                              (eff := [[]]); try (reflexivity).
     + apply eval_funid.
     + intros. inversion H.
@@ -49,23 +49,23 @@ Proof.
       ** inversion H1.
     + simpl. reflexivity.
     + eapply eval_apply with (vals := [VEmptyTuple]) 
-                             (body := (EApply (EFunId ("x"%string, 1)) [EVar "X"%string])) (n := 0)
+                             (body := (EApp (EFunId ("x"%string, 1)) [EVar "X"%string])) (n := 0)
                              (var_list := ["X"%string]) 
                              (ref := []) (ids := [1])
                              (ext := [(1, ("x"%string, 1), 
-                                     (["X"%string], EApply (EFunId ("x"%string, 1)) [EVar "X"%string]))]) 
+                                     (["X"%string], EApp (EFunId ("x"%string, 1)) [EVar "X"%string]))]) 
                              (eff := [[]]); try (reflexivity).
 Admitted.
 
 (* This is not accepted by the compiler in Core Erlang *)
 Example eval_letrec2 : 
   |[], 0, ELet ["F"%string] [EFun ["X"%string] 
-         (EApply (EVar "F"%string) [EVar "X"%string])] 
-            (EApply (EVar "F"%string) [EEmptyTuple]), []| 
+         (EApp (EVar "F"%string) [EVar "X"%string])] 
+            (EApp (EVar "F"%string) [EEmptyTuple]), []| 
 -e>
 |1, inr novar, []|.
 Proof.
-  eapply eval_let with (vals := [VClosure [] [] 0 ["X"%string] (EApply (EVar "F"%string) [EVar "X"%string])]) 
+  eapply eval_let with (vals := [VClos [] [] 0 ["X"%string] (EApp (EVar "F"%string) [EVar "X"%string])]) 
                        (ids := [1])
                        (eff := [[]]); auto.
   * simpl. intros. inversion H.
@@ -74,7 +74,7 @@ Proof.
   * reflexivity.
   * simpl. eapply eval_apply with (vals := [VEmptyTuple]) (n := 0)
                                   (var_list := ["X"%string]) (ids := [1])
-                                  (body := (EApply (EVar "F"%string) [EVar "X"%string])) 
+                                  (body := (EApp (EVar "F"%string) [EVar "X"%string])) 
                                   (ref := []) (ext := []) (eff := [[]]); try(reflexivity).
     - apply eval_var.
     - intros. inversion H.
@@ -88,146 +88,146 @@ Proof.
 Qed.
 
 (* Top level functions, and their closures must be added initially *)
-Example multiple_top_level_funs : |[(inr ("fun1"%string, 0), VClosure [] [
-    (0, ("fun1"%string, 0), ([], (EApply (EFunId ("fun3"%string, 0)) [])));
-    (1, ("fun2"%string, 0), ([], (ELiteral (Integer 42))));
-    (2, ("fun3"%string, 0), ([], (EApply (EFunId ("fun2"%string, 0)) [])))
-  ] 0 [] (EApply (EFunId ("fun3"%string, 0)) [])) ; 
-                                      (inr ("fun2"%string, 0), VClosure [] [
-    (0, ("fun1"%string, 0), ([], (EApply (EFunId ("fun3"%string, 0)) [])));
-    (1, ("fun2"%string, 0), ([], (ELiteral (Integer 42))));
-    (2, ("fun3"%string, 0), ([], (EApply (EFunId ("fun2"%string, 0)) [])))
-  ] 1 [] (ELiteral (Integer 42))) ;
-                                      (inr ("fun3"%string, 0), VClosure [] [
-    (0, ("fun1"%string, 0), ([], (EApply (EFunId ("fun3"%string, 0)) [])));
-    (1, ("fun2"%string, 0), ([], (ELiteral (Integer 42))));
-    (2, ("fun3"%string, 0), ([], (EApply (EFunId ("fun2"%string, 0)) [])))
-  ] 2 [] (EApply (EFunId ("fun2"%string, 0)) []))], 3
-                                      , EApply (EFunId ("fun1"%string,0)) [], []| 
+Example multiple_top_level_funs : |[(inr ("fun1"%string, 0), VClos [] [
+    (0, ("fun1"%string, 0), ([], (EApp (EFunId ("fun3"%string, 0)) [])));
+    (1, ("fun2"%string, 0), ([], (ELit (Integer 42))));
+    (2, ("fun3"%string, 0), ([], (EApp (EFunId ("fun2"%string, 0)) [])))
+  ] 0 [] (EApp (EFunId ("fun3"%string, 0)) [])) ; 
+                                      (inr ("fun2"%string, 0), VClos [] [
+    (0, ("fun1"%string, 0), ([], (EApp (EFunId ("fun3"%string, 0)) [])));
+    (1, ("fun2"%string, 0), ([], (ELit (Integer 42))));
+    (2, ("fun3"%string, 0), ([], (EApp (EFunId ("fun2"%string, 0)) [])))
+  ] 1 [] (ELit (Integer 42))) ;
+                                      (inr ("fun3"%string, 0), VClos [] [
+    (0, ("fun1"%string, 0), ([], (EApp (EFunId ("fun3"%string, 0)) [])));
+    (1, ("fun2"%string, 0), ([], (ELit (Integer 42))));
+    (2, ("fun3"%string, 0), ([], (EApp (EFunId ("fun2"%string, 0)) [])))
+  ] 2 [] (EApp (EFunId ("fun2"%string, 0)) []))], 3
+                                      , EApp (EFunId ("fun1"%string,0)) [], []| 
 -e> 
-  |3, inl (VLiteral (Integer 42)), []|.
+  |3, inl (VLit (Integer 42)), []|.
 Proof.
   remember [
-  (0, ("fun1"%string, 0), ([], (EApply (EFunId ("fun3"%string, 0)) [])));
-  (1, ("fun2"%string, 0), ([], (ELiteral (Integer 42))));
-  (2, ("fun3"%string, 0), ([], (EApply (EFunId ("fun2"%string, 0)) [])))
+  (0, ("fun1"%string, 0), ([], (EApp (EFunId ("fun3"%string, 0)) [])));
+  (1, ("fun2"%string, 0), ([], (ELit (Integer 42))));
+  (2, ("fun3"%string, 0), ([], (EApp (EFunId ("fun2"%string, 0)) [])))
 ] as ext.
   eapply eval_apply with (vals := []) (ref := []) (ext := ext) (eff := [])
-                         (body := (EApply (EFunId ("fun3"%string, 0)) [])) 
+                         (body := (EApp (EFunId ("fun3"%string, 0)) [])) 
                          (var_list := []) (n := 0) (ids := []); auto.
   * apply eval_funid.
   * simpl. intros. inversion H.
   * reflexivity.
   * simpl. eapply eval_apply with (vals := []) (n := 2) (ref := []) (ext := ext) (eff := [])
-                                 (body := (EApply (EFunId ("fun2"%string, 0)) [])) 
+                                 (body := (EApp (EFunId ("fun2"%string, 0)) [])) 
                                  (var_list := []) (ids := []); auto.
     - rewrite Heqext. simpl. apply eval_funid.
     - intros. inversion H.
     - simpl. reflexivity.
     - simpl. eapply eval_apply with (vals := []) (n := 1) (ref := []) (ext := ext) (eff := [])
-                                    (body := (ELiteral (Integer 42))) (var_list := []) (ids := []); auto.
+                                    (body := (ELit (Integer 42))) (var_list := []) (ids := []); auto.
       + rewrite Heqext. apply eval_funid.
       + intros. inversion H.
       + reflexivity.
       + apply eval_lit.
 Qed.
 
-Example weird_apply : |[], 0, ELetrec [("f"%string, 1)] [["X"%string]]
+Example weird_apply : |[], 0, ELetRec [("f"%string, 1)] [["X"%string]]
    [ECase (EVar "X"%string)
-          [PLiteral (Integer 0) ; PLiteral (Integer 1); PVar "X"%string]
-          [ELiteral (Atom "true"%string); ELiteral (Atom "true"%string); ELiteral (Atom "true"%string)]
-          [ELiteral (Integer 5);
-           EApply (EFunId ("f"%string, 1)) [ELiteral (Integer 0)];
-           EApply (EFunId ("f"%string, 1)) [ELiteral (Integer 1)]
+          [PLit (Integer 0) ; PLit (Integer 1); PVar "X"%string]
+          [ELit (Atom "true"%string); ELit (Atom "true"%string); ELit (Atom "true"%string)]
+          [ELit (Integer 5);
+           EApp (EFunId ("f"%string, 1)) [ELit (Integer 0)];
+           EApp (EFunId ("f"%string, 1)) [ELit (Integer 1)]
           ]
    ]
    (ELet ["X"%string] [EFun ["F"%string]
-       (ELetrec [("f"%string, 1)] [["X"%string]] [ELiteral (Integer 0)] 
-          (EApply (EVar "F"%string) [ELiteral (Integer 2)])
+       (ELetRec [("f"%string, 1)] [["X"%string]] [ELit (Integer 0)] 
+          (EApp (EVar "F"%string) [ELit (Integer 2)])
        )
      ]
-    (EApply (EVar "X"%string) [EFunId ("f"%string, 1)])
+    (EApp (EVar "X"%string) [EFunId ("f"%string, 1)])
    ), []|
 -e> 
-  |3, inl (VLiteral (Integer 5)), []|.
+  |3, inl (VLit (Integer 5)), []|.
 Proof.
   eapply eval_letrec; auto.
   simpl. eapply eval_let with (vals := [
- VClosure 
+ VClos 
   [(inr ("f"%string, 1),
-   VClosure []
+   VClos []
      [(0, ("f"%string, 1),
       (["X"%string],
       ECase (EVar "X"%string)
-        [PLiteral (Integer 0); PLiteral (Integer 1); PVar "X"%string]
-        [ELiteral (Atom "true"); ELiteral (Atom "true"); ELiteral (Atom "true")]
-        [ELiteral (Integer 5); EApply (EFunId ("f"%string, 1)) [ELiteral (Integer 0)];
-        EApply (EFunId ("f"%string, 1)) [ELiteral (Integer 1)]]))] 0 ["X"%string]
+        [PLit (Integer 0); PLit (Integer 1); PVar "X"%string]
+        [ELit (Atom "true"); ELit (Atom "true"); ELit (Atom "true")]
+        [ELit (Integer 5); EApp (EFunId ("f"%string, 1)) [ELit (Integer 0)];
+        EApp (EFunId ("f"%string, 1)) [ELit (Integer 1)]]))] 0 ["X"%string]
      (ECase (EVar "X"%string)
-        [PLiteral (Integer 0); PLiteral (Integer 1); PVar "X"%string]
-        [ELiteral (Atom "true"); ELiteral (Atom "true"); ELiteral (Atom "true")]
-        [ELiteral (Integer 5); EApply (EFunId ("f"%string, 1)) [ELiteral (Integer 0)];
-        EApply (EFunId ("f"%string, 1)) [ELiteral (Integer 1)]]))
+        [PLit (Integer 0); PLit (Integer 1); PVar "X"%string]
+        [ELit (Atom "true"); ELit (Atom "true"); ELit (Atom "true")]
+        [ELit (Integer 5); EApp (EFunId ("f"%string, 1)) [ELit (Integer 0)];
+        EApp (EFunId ("f"%string, 1)) [ELit (Integer 1)]]))
   ]
   [] 1
   ["F"%string]
-  (ELetrec [("f"%string, 1)] [["X"%string]] [ELiteral (Integer 0)]
-        (EApply (EVar "F"%string) [ELiteral (Integer 2)]))
+  (ELetRec [("f"%string, 1)] [["X"%string]] [ELit (Integer 0)]
+        (EApp (EVar "F"%string) [ELit (Integer 2)]))
  ]
   ) (eff := [[]]) (ids := [2]); auto.
   * intros. inversion H; inversion H1. unfold append_funs_to_env. simpl. apply eval_fun.
   * simpl. eapply eval_apply with (var_list := ["F"%string]) (n := 1) (eff := [[]]) (ids := [2])
-  (vals := [VClosure []
+  (vals := [VClos []
      [(0, ("f"%string, 1),
       (["X"%string],
       ECase (EVar "X"%string)
-        [PLiteral (Integer 0); PLiteral (Integer 1); PVar "X"%string]
-        [ELiteral (Atom "true"); ELiteral (Atom "true"); ELiteral (Atom "true")]
-        [ELiteral (Integer 5); EApply (EFunId ("f"%string, 1)) [ELiteral (Integer 0)];
-        EApply (EFunId ("f"%string, 1)) [ELiteral (Integer 1)]]))] 0 ["X"%string]
+        [PLit (Integer 0); PLit (Integer 1); PVar "X"%string]
+        [ELit (Atom "true"); ELit (Atom "true"); ELit (Atom "true")]
+        [ELit (Integer 5); EApp (EFunId ("f"%string, 1)) [ELit (Integer 0)];
+        EApp (EFunId ("f"%string, 1)) [ELit (Integer 1)]]))] 0 ["X"%string]
      (ECase (EVar "X"%string)
-        [PLiteral (Integer 0); PLiteral (Integer 1); PVar "X"%string]
-        [ELiteral (Atom "true"); ELiteral (Atom "true"); ELiteral (Atom "true")]
-        [ELiteral (Integer 5); EApply (EFunId ("f"%string, 1)) [ELiteral (Integer 0)];
-        EApply (EFunId ("f"%string, 1)) [ELiteral (Integer 1)]])])
-  (body := (ELetrec [("f"%string, 1)] [["X"%string]] [ELiteral (Integer 0)]
-       (EApply (EVar "F"%string) [ELiteral (Integer 2)])))
+        [PLit (Integer 0); PLit (Integer 1); PVar "X"%string]
+        [ELit (Atom "true"); ELit (Atom "true"); ELit (Atom "true")]
+        [ELit (Integer 5); EApp (EFunId ("f"%string, 1)) [ELit (Integer 0)];
+        EApp (EFunId ("f"%string, 1)) [ELit (Integer 1)]])])
+  (body := (ELetRec [("f"%string, 1)] [["X"%string]] [ELit (Integer 0)]
+       (EApp (EVar "F"%string) [ELit (Integer 2)])))
   (ref := [(inr ("f"%string, 1),
-     VClosure []
+     VClos []
        [(0, ("f"%string, 1),
         (["X"%string],
         ECase (EVar "X"%string)
-          [PLiteral (Integer 0); PLiteral (Integer 1); PVar "X"%string]
-          [ELiteral (Atom "true"); ELiteral (Atom "true"); ELiteral (Atom "true")]
-          [ELiteral (Integer 5); EApply (EFunId ("f"%string, 1)) [ELiteral (Integer 0)];
-          EApply (EFunId ("f"%string, 1)) [ELiteral (Integer 1)]]))] 0 ["X"%string]
+          [PLit (Integer 0); PLit (Integer 1); PVar "X"%string]
+          [ELit (Atom "true"); ELit (Atom "true"); ELit (Atom "true")]
+          [ELit (Integer 5); EApp (EFunId ("f"%string, 1)) [ELit (Integer 0)];
+          EApp (EFunId ("f"%string, 1)) [ELit (Integer 1)]]))] 0 ["X"%string]
        (ECase (EVar "X"%string)
-          [PLiteral (Integer 0); PLiteral (Integer 1); PVar "X"%string]
-          [ELiteral (Atom "true"); ELiteral (Atom "true"); ELiteral (Atom "true")]
-          [ELiteral (Integer 5); EApply (EFunId ("f"%string, 1)) [ELiteral (Integer 0)];
-          EApply (EFunId ("f"%string, 1)) [ELiteral (Integer 1)]]))])
+          [PLit (Integer 0); PLit (Integer 1); PVar "X"%string]
+          [ELit (Atom "true"); ELit (Atom "true"); ELit (Atom "true")]
+          [ELit (Integer 5); EApp (EFunId ("f"%string, 1)) [ELit (Integer 0)];
+          EApp (EFunId ("f"%string, 1)) [ELit (Integer 1)]]))])
   (ext := []); auto.
     - apply eval_var.
     - intros. inversion H; inversion H1. simpl. apply eval_funid.
     - simpl. eapply eval_letrec; auto. simpl.
       eapply eval_apply with (var_list := ["X"%string]) (eff := [[]])
-        (vals := [VLiteral (Integer 2)])
+        (vals := [VLit (Integer 2)])
         (ref := []) (n := 0) (ids := [3])
         (body := (ECase (EVar "X"%string)
-       [PLiteral (Integer 0); PLiteral (Integer 1); PVar "X"%string]
-       [ELiteral (Atom "true"); ELiteral (Atom "true"); ELiteral (Atom "true")]
-       [ELiteral (Integer 5); EApply (EFunId ("f"%string, 1)) [ELiteral (Integer 0)];
-       EApply (EFunId ("f"%string, 1)) [ELiteral (Integer 1)]]))
+       [PLit (Integer 0); PLit (Integer 1); PVar "X"%string]
+       [ELit (Atom "true"); ELit (Atom "true"); ELit (Atom "true")]
+       [ELit (Integer 5); EApp (EFunId ("f"%string, 1)) [ELit (Integer 0)];
+       EApp (EFunId ("f"%string, 1)) [ELit (Integer 1)]]))
         (ext := [(0, ("f"%string, 1),
      (["X"%string],
      ECase (EVar "X"%string)
-       [PLiteral (Integer 0); PLiteral (Integer 1); PVar "X"%string]
-       [ELiteral (Atom "true"); ELiteral (Atom "true"); ELiteral (Atom "true")]
-       [ELiteral (Integer 5); EApply (EFunId ("f"%string, 1)) [ELiteral (Integer 0)];
-       EApply (EFunId ("f"%string, 1)) [ELiteral (Integer 1)]]))]); auto.
+       [PLit (Integer 0); PLit (Integer 1); PVar "X"%string]
+       [ELit (Atom "true"); ELit (Atom "true"); ELit (Atom "true")]
+       [ELit (Integer 5); EApp (EFunId ("f"%string, 1)) [ELit (Integer 0)];
+       EApp (EFunId ("f"%string, 1)) [ELit (Integer 1)]]))]); auto.
       + apply eval_var.
       + intros. inversion H; inversion H1. apply eval_lit.
-      + simpl. eapply eval_case with (i := 2) (v := VLiteral (Integer 2)); auto.
+      + simpl. eapply eval_case with (i := 2) (v := VLit (Integer 2)); auto.
         ** apply eval_var.
         ** simpl. reflexivity.
         ** intros. inversion H.
@@ -238,23 +238,23 @@ Proof.
         ** simpl. apply eval_lit.
         ** simpl. eapply eval_apply with (var_list := ["X"%string])
                      (eff := [[]]) (n := 0) (ids := [3])
-                     (vals := [VLiteral (Integer 1)])
+                     (vals := [VLit (Integer 1)])
                      (body := (ECase (EVar "X"%string)
-                                [PLiteral (Integer 0); PLiteral (Integer 1); PVar "X"%string]
-                                [ELiteral (Atom "true"); ELiteral (Atom "true"); ELiteral (Atom "true")]
-                                [ELiteral (Integer 5); EApply (EFunId ("f"%string, 1)) [ELiteral (Integer 0)];
-                                EApply (EFunId ("f"%string, 1)) [ELiteral (Integer 1)]]))
+                                [PLit (Integer 0); PLit (Integer 1); PVar "X"%string]
+                                [ELit (Atom "true"); ELit (Atom "true"); ELit (Atom "true")]
+                                [ELit (Integer 5); EApp (EFunId ("f"%string, 1)) [ELit (Integer 0)];
+                                EApp (EFunId ("f"%string, 1)) [ELit (Integer 1)]]))
                      (ref := [])
                      (ext := [(0, ("f"%string, 1),
                               (["X"%string],
                               ECase (EVar "X"%string)
-                                [PLiteral (Integer 0); PLiteral (Integer 1); PVar "X"%string]
-                                [ELiteral (Atom "true"); ELiteral (Atom "true"); ELiteral (Atom "true")]
-                                [ELiteral (Integer 5); EApply (EFunId ("f"%string, 1)) [ELiteral (Integer 0)];
-                                EApply (EFunId ("f"%string, 1)) [ELiteral (Integer 1)]]))]); auto.
+                                [PLit (Integer 0); PLit (Integer 1); PVar "X"%string]
+                                [ELit (Atom "true"); ELit (Atom "true"); ELit (Atom "true")]
+                                [ELit (Integer 5); EApp (EFunId ("f"%string, 1)) [ELit (Integer 0)];
+                                EApp (EFunId ("f"%string, 1)) [ELit (Integer 1)]]))]); auto.
          -- apply eval_funid.
          -- intros. inversion H; inversion H1. apply eval_lit.
-         -- simpl. eapply eval_case with (i := 1) (v := VLiteral (Integer 1)); auto.
+         -- simpl. eapply eval_case with (i := 1) (v := VLit (Integer 1)); auto.
            ++ apply eval_var.
            ++ simpl. auto.
            ++ simpl. reflexivity.
@@ -263,25 +263,25 @@ Proof.
              *** inversion H2.
            ++ simpl. apply eval_lit.
            ++ eapply eval_apply with (var_list := ["X"%string])
-                     (vals := [VLiteral (Integer 0)])
+                     (vals := [VLit (Integer 0)])
                      (eff := [[]]) (n := 0) (ids := [3])
                      (body := (ECase (EVar "X"%string)
-                                [PLiteral (Integer 0); PLiteral (Integer 1); PVar "X"%string]
-                                [ELiteral (Atom "true"); ELiteral (Atom "true"); ELiteral (Atom "true")]
-                                [ELiteral (Integer 5); EApply (EFunId ("f"%string, 1)) [ELiteral (Integer 0)];
-                                EApply (EFunId ("f"%string, 1)) [ELiteral (Integer 1)]]))
+                                [PLit (Integer 0); PLit (Integer 1); PVar "X"%string]
+                                [ELit (Atom "true"); ELit (Atom "true"); ELit (Atom "true")]
+                                [ELit (Integer 5); EApp (EFunId ("f"%string, 1)) [ELit (Integer 0)];
+                                EApp (EFunId ("f"%string, 1)) [ELit (Integer 1)]]))
                      (ref := [])
                      (ext := [(0, ("f"%string, 1),
                               (["X"%string],
                               ECase (EVar "X"%string)
-                                [PLiteral (Integer 0); PLiteral (Integer 1); PVar "X"%string]
-                                [ELiteral (Atom "true"); ELiteral (Atom "true"); ELiteral (Atom "true")]
-                                [ELiteral (Integer 5); EApply (EFunId ("f"%string, 1)) [ELiteral (Integer 0)];
-                                EApply (EFunId ("f"%string, 1)) [ELiteral (Integer 1)]]))]); auto.
+                                [PLit (Integer 0); PLit (Integer 1); PVar "X"%string]
+                                [ELit (Atom "true"); ELit (Atom "true"); ELit (Atom "true")]
+                                [ELit (Integer 5); EApp (EFunId ("f"%string, 1)) [ELit (Integer 0)];
+                                EApp (EFunId ("f"%string, 1)) [ELit (Integer 1)]]))]); auto.
              *** simpl. apply eval_funid.
              *** intros. inversion H; inversion H1. apply eval_lit.
              *** reflexivity.
-             *** simpl. eapply eval_case with (i := 0) (v := VLiteral (Integer 0)); auto.
+             *** simpl. eapply eval_case with (i := 0) (v := VLit (Integer 0)); auto.
                --- apply eval_var.
                --- simpl. auto.
                --- simpl. reflexivity.
@@ -293,20 +293,20 @@ Qed.
 
 Example top_overwrite : 
   |[(inr ("fun2"%string, 0), 
-       VClosure [] [(0, ("fun2"%string, 0),([],  (ELiteral (Integer 42)) ))] 0 [] (ELiteral (Integer 42)))], 1,
-  ELetrec [("fun2"%string, 0)] [[]] [ELiteral (Integer 40)] 
-     (EApply (EFunId ("fun2"%string, 0)) []), [] | 
+       VClos [] [(0, ("fun2"%string, 0),([],  (ELit (Integer 42)) ))] 0 [] (ELit (Integer 42)))], 1,
+  ELetRec [("fun2"%string, 0)] [[]] [ELit (Integer 40)] 
+     (EApp (EFunId ("fun2"%string, 0)) []), [] | 
 -e>
-  |2, inl (VLiteral (Integer 40)), []|.
+  |2, inl (VLit (Integer 40)), []|.
 Proof.
   eapply eval_letrec; auto.
   * unfold append_funs_to_env. simpl. eapply eval_apply with (vals := []) (eff := []) (n := 1) (ids := [])
-                                  (ref := [(inr ("fun2"%string, 0), VClosure [] 
+                                  (ref := [(inr ("fun2"%string, 0), VClos [] 
                                                                     [(0, ("fun2"%string, 0), 
-                                                                    ([], ELiteral (Integer 42)))] 0 []
-                                                                    (ELiteral (Integer 42)))]) 
-                                  (ext := [(1, ("fun2"%string, 0), ([],  (ELiteral (Integer 40)) ))]) 
-                                  (body := (ELiteral (Integer 40))) (var_list := []); auto.
+                                                                    ([], ELit (Integer 42)))] 0 []
+                                                                    (ELit (Integer 42)))]) 
+                                  (ext := [(1, ("fun2"%string, 0), ([],  (ELit (Integer 40)) ))]) 
+                                  (body := (ELit (Integer 40))) (var_list := []); auto.
     - unfold append_funs_to_env. simpl. apply eval_funid.
     - intros. inversion H.
     - apply eval_lit.
@@ -315,17 +315,17 @@ Qed.
 
 Example top_no_overwrite : 
   |[(inr ("fun2"%string, 0), 
-     VClosure [] [(("fun2"%string, 0), ([], ELiteral (Integer 42)))] 0 [] (ELiteral (Integer 42)))],
-   ELetrec [("fun2"%string, 1)] [["X"%string]] [(ELiteral (Integer 40))] 
-     (EApply (EFunId ("fun2"%string, 0)) []), [] |
+     VClos [] [(("fun2"%string, 0), ([], ELit (Integer 42)))] 0 [] (ELit (Integer 42)))],
+   ELetRec [("fun2"%string, 1)] [["X"%string]] [(ELit (Integer 40))] 
+     (EApp (EFunId ("fun2"%string, 0)) []), [] |
 -e> 
-  |inl (VLiteral (Integer 42)), []|.
+  |inl (VLit (Integer 42)), []|.
 Proof.
   eapply eval_letrec; auto.
   * simpl. eapply eval_apply with (vals := []) (n := 0)
                                   (ref := [])
-                                  (ext := [("fun2"%string, 0, ([], ELiteral (Integer 42)))]) 
-                                  (body := ELiteral (Integer 42)) 
+                                  (ext := [("fun2"%string, 0, ([], ELit (Integer 42)))]) 
+                                  (body := ELit (Integer 42)) 
                                   (var_list := [])
                                   (eff := []); auto.
     - apply eval_funid.
@@ -336,14 +336,14 @@ Qed.
 
 (** This is not accepted by the compiler in Core Erlang *)
 Example eval_let_func : 
-  |[(inl "X"%string, VLiteral (Integer 42))], 
-   ELet ["X"%string; "X"%string] [EFun [] (EEmptyList); EFun [] (EEmptyMap)] 
+  |[(inl "X"%string, VLit (Integer 42))], 
+   ELet ["X"%string; "X"%string] [EFun [] (ENil); EFun [] (EEmptyMap)] 
      (EEmptyMap), []| 
 -e> 
   |inl (VEmptyMap), []|.
 Proof.
-  eapply eval_let with (vals := [VClosure [(inl "X"%string, VLiteral (Integer 42))] [] 0 [] (EEmptyList); 
-                                 VClosure [(inl "X"%string, VLiteral (Integer 42))] [] 0 [] (EEmptyMap)])
+  eapply eval_let with (vals := [VClos [(inl "X"%string, VLit (Integer 42))] [] 0 [] (ENil); 
+                                 VClos [(inl "X"%string, VLit (Integer 42))] [] 0 [] (EEmptyMap)])
                        (eff := [[]; []]); auto.
   * simpl. intros. inversion H.
     - apply eval_fun.
@@ -357,13 +357,13 @@ Proof.
 Qed.
 
 Example eval_let_apply : 
-  |[(inl "X"%string, VLiteral (Integer 42))], 
+  |[(inl "X"%string, VLit (Integer 42))], 
    ELet ["Y"%string] [EFun [] (EVar "X"%string)] 
-     (EApply (EVar "Y"%string) []), []| 
+     (EApp (EVar "Y"%string) []), []| 
 -e> 
-  |inl (VLiteral (Integer 42)), []|.
+  |inl (VLit (Integer 42)), []|.
 Proof.
-  eapply eval_let with (vals := [VClosure [(inl "X"%string, VLiteral (Integer 42))] [] 0 [] 
+  eapply eval_let with (vals := [VClos [(inl "X"%string, VLit (Integer 42))] [] 0 [] 
                                           (EVar "X"%string)])
                        (eff := [[]]); auto.
   * simpl. intros. inversion H.
@@ -371,7 +371,7 @@ Proof.
     - inversion H1.
   * reflexivity.
   * simpl. eapply eval_apply with (vals := []) (n := 0)
-                                  (ref := [(inl "X"%string, VLiteral (Integer 42))]) 
+                                  (ref := [(inl "X"%string, VLit (Integer 42))]) 
                                   (ext := []) 
                                   (body := (EVar "X"%string)) 
                                   (var_list := [])
@@ -383,18 +383,18 @@ Proof.
 Qed.
 
 Example eval_muliple_let : 
-  |[], ELet ["X"%string] [ELiteral (Integer 1)] 
-         (ELet ["X"%string] [ELiteral (Integer 2)] 
+  |[], ELet ["X"%string] [ELit (Integer 1)] 
+         (ELet ["X"%string] [ELit (Integer 2)] 
             (EVar "X"%string)), []| 
 -e> 
-  |inl (VLiteral (Integer 2)), []|.
+  |inl (VLit (Integer 2)), []|.
 Proof.
-  eapply eval_let with (vals := [VLiteral (Integer 1)]) (eff := [[]]); auto.
+  eapply eval_let with (vals := [VLit (Integer 1)]) (eff := [[]]); auto.
   * intros. inversion H.
     - apply eval_lit.
     - inversion H1.
   * simpl. reflexivity.
-  * eapply eval_let with (vals := [VLiteral (Integer 2)]) (eff := [[]]); auto.
+  * eapply eval_let with (vals := [VLit (Integer 2)]) (eff := [[]]); auto.
     - simpl. intros. inversion H.
       + apply eval_lit.
       + inversion H1.
@@ -435,12 +435,12 @@ Qed.
 (** This shouldn't compile in Core Erlang *)
 Example eval_let_3 : 
   |[(inl "X"%string, VEmptyMap)],
-   ELet ["X"%string; "X"%string; "Y"%string] [EEmptyTuple; EEmptyList; EVar "X"%string] 
+   ELet ["X"%string; "X"%string; "Y"%string] [EEmptyTuple; ENil; EVar "X"%string] 
      (EVar "Y"%string), []|
 -e>
   |inl (VEmptyMap), []|.
 Proof.
-  eapply eval_let with (vals := [(VEmptyTuple) ; (VEmptyList); (VEmptyMap)]) 
+  eapply eval_let with (vals := [(VEmptyTuple) ; (VNil); (VEmptyMap)]) 
                        (eff := [[];[];[]]); auto.
   * simpl. intros. inversion H.
     - apply eval_var.
@@ -454,11 +454,11 @@ Proof.
 Qed.
 
 Example let_eval_4 : 
-  |[], ELet ["X"%string] [ELiteral (Integer 5)] (EVar "X"%string), []| 
+  |[], ELet ["X"%string] [ELit (Integer 5)] (EVar "X"%string), []| 
 -e> 
-  | inl (VLiteral (Integer 5)), []|.
+  | inl (VLit (Integer 5)), []|.
 Proof.
-  eapply eval_let with (vals := [VLiteral (Integer 5)]) (eff := [[]]); auto.
+  eapply eval_let with (vals := [VLit (Integer 5)]) (eff := [[]]); auto.
   * intros. simpl in *. inversion H.
     - apply eval_lit.
     - inversion H1.
@@ -467,11 +467,11 @@ Proof.
 Qed.
 
 Example tuple_eval : 
-  |[(inl "X"%string, VLiteral (Atom "asd"%string)); 
+  |[(inl "X"%string, VLit (Atom "asd"%string)); 
     (inl "Y"%string, VEmptyTuple)], 
-   ETuple [ELiteral (Integer 5); EVar "X"%string; EVar "Y"%string], []| 
+   ETuple [ELit (Integer 5); EVar "X"%string; EVar "Y"%string], []| 
 -e>
-  |inl (VTuple [VLiteral (Integer 5); VLiteral (Atom "asd"%string); VEmptyTuple]), []|.
+  |inl (VTuple [VLit (Integer 5); VLit (Atom "asd"%string); VEmptyTuple]), []|.
 Proof.
   eapply eval_tuple with (eff := [[];[];[]]); auto.
   * intros. inversion H.
@@ -485,20 +485,20 @@ Qed.
 
 Example apply_top_eval : 
   |[(inr ("Plus"%string, 2), 
-       VClosure [] [(("Plus"%string, 2),
-                     (["X"%string ; "Y"%string], ELiteral (Integer 3)))] 
+       VClos [] [(("Plus"%string, 2),
+                     (["X"%string ; "Y"%string], ELit (Integer 3)))] 
                 0 ["X"%string ; "Y"%string] 
-                (ELiteral (Integer 3)))], 
-   EApply (EFunId ("Plus"%string, 2)) [ELiteral (Integer 2); ELiteral (Integer 3)], []|
+                (ELit (Integer 3)))], 
+   EApp (EFunId ("Plus"%string, 2)) [ELit (Integer 2); ELit (Integer 3)], []|
 -e>
-  |inl ((VLiteral (Integer 3))), []|.
+  |inl ((VLit (Integer 3))), []|.
 Proof.
-  eapply eval_apply with (vals := [VLiteral (Integer 2) ; VLiteral (Integer 3)])
+  eapply eval_apply with (vals := [VLit (Integer 2) ; VLit (Integer 3)])
                          (var_list := ["X"%string; "Y"%string]) 
-                         (body := ELiteral (Integer 3)) 
+                         (body := ELit (Integer 3)) 
                          (ref := []) (n := 0)
                          (ext := [(("Plus"%string, 2),
-                                   (["X"%string ; "Y"%string], ELiteral (Integer 3)))])
+                                   (["X"%string ; "Y"%string], ELit (Integer 3)))])
                          (eff := [[];[]]); auto.
   * apply eval_funid.
   * simpl. intros. inversion H.
@@ -512,15 +512,15 @@ Qed.
 
 Example apply_eval : 
   |[(inl "Minus"%string,
-      VClosure [] [] 0 ["X"%string; "Y"%string] (ELiteral (Integer 42))) ; 
+      VClos [] [] 0 ["X"%string; "Y"%string] (ELit (Integer 42))) ; 
     (inl "X"%string, VEmptyMap)], 
-   EApply (EVar "Minus"%string) [EVar "X"%string; EVar "X"%string], []|
+   EApp (EVar "Minus"%string) [EVar "X"%string; EVar "X"%string], []|
 -e>
-  |inl (VLiteral (Integer 42)), []|.
+  |inl (VLit (Integer 42)), []|.
 Proof.
   eapply eval_apply with (vals := [VEmptyMap; VEmptyMap]) 
                          (var_list := ["X"%string; "Y"%string]) 
-                         (body := (ELiteral (Integer 42))) (n := 0)
+                         (body := (ELit (Integer 42))) (n := 0)
                          (ref := []) (ext := []) (eff := [[];[]]); auto.
   * apply eval_var.
   * simpl. intros. inversion H.
@@ -534,10 +534,10 @@ Qed.
 
 
 Example list_eval : 
-  |[(inl "X"%string, VLiteral (Integer 5))],
-   EList (EVar "X"%string) (EEmptyList), []| 
+  |[(inl "X"%string, VLit (Integer 5))],
+   ECons (EVar "X"%string) (ENil), []| 
 -e>
-  | inl (VList (VLiteral (Integer 5)) (VEmptyList)), []|.
+  | inl (VCons (VLit (Integer 5)) (VNil)), []|.
 Proof.
   eapply eval_list.
   * instantiate (1 := []). rewrite app_nil_r. reflexivity.
@@ -546,14 +546,14 @@ Proof.
 Qed.
 
 Example list_eval2 : 
-  |[(inl "X"%string, VLiteral (Integer 5))], 
-   EList (EVar "X"%string) 
-         (EList (EVar "X"%string) 
-                (EEmptyList)), []| 
+  |[(inl "X"%string, VLit (Integer 5))], 
+   ECons (EVar "X"%string) 
+         (ECons (EVar "X"%string) 
+                (ENil)), []| 
 -e> 
-  |inl (VList (VLiteral (Integer 5)) 
-              (VList (VLiteral (Integer 5)) 
-                     (VEmptyList))), []|.
+  |inl (VCons (VLit (Integer 5)) 
+              (VCons (VLit (Integer 5)) 
+                     (VNil))), []|.
 Proof.
   eapply eval_list with (eff2 := []).
   * reflexivity.
@@ -566,17 +566,17 @@ Qed.
 
 Example let_eval_overwrite : 
   |[], ELet ["X"%string] [EFun [] (EEmptyTuple)] 
-         (ELet ["X"%string] [ELiteral (Integer 5)] 
+         (ELet ["X"%string] [ELit (Integer 5)] 
             (EVar "X"%string)), []|
 -e>
-  |inl (VLiteral (Integer 5)), []|.
+  |inl (VLit (Integer 5)), []|.
 Proof.
-  eapply eval_let with (vals := [VClosure [] [] 0 [] (EEmptyTuple)]) (eff := [[]]); auto.
+  eapply eval_let with (vals := [VClos [] [] 0 [] (EEmptyTuple)]) (eff := [[]]); auto.
   * simpl. intros. inversion H.
     - apply eval_fun.
     - inversion H1.
   * reflexivity.
-  * simpl. eapply eval_let with (vals := [VLiteral (Integer 5)]) (eff := [[]]); auto.
+  * simpl. eapply eval_let with (vals := [VLit (Integer 5)]) (eff := [[]]); auto.
     - simpl. intros. inversion H.
       + apply eval_lit.
       + inversion H1.
@@ -585,12 +585,12 @@ Proof.
 Qed.
 
 Example map_eval :
-  |[(inl "X"%string, VLiteral (Integer 42))], 
-    EMap [ELiteral (Integer 5)] [EVar "X"%string], []|
+  |[(inl "X"%string, VLit (Integer 42))], 
+    EMap [ELit (Integer 5)] [EVar "X"%string], []|
 -e>
-  |inl (VMap [VLiteral (Integer 5)] [VLiteral (Integer 42)]), []|.
+  |inl (VMap [VLit (Integer 5)] [VLit (Integer 42)]), []|.
 Proof.
-  eapply eval_map with (kvals := [VLiteral (Integer 5)]) (vvals := [VLiteral (Integer 42)]) 
+  eapply eval_map with (kvals := [VLit (Integer 5)]) (vvals := [VLit (Integer 42)]) 
                        (eff := [[];[]]); auto.
   * intros. inversion H.
     - subst. apply eval_lit.
@@ -601,15 +601,15 @@ Proof.
 Qed.
 
 Example map_eval2 : 
-  |[(inl "X"%string, VLiteral (Integer 42))], 
-   EMap [ELiteral (Integer 54); EVar "X"%string] 
+  |[(inl "X"%string, VLit (Integer 42))], 
+   EMap [ELit (Integer 54); EVar "X"%string] 
         [EVar "X"%string; EVar "X"%string], []|
 -e> 
-  |inl (VMap [VLiteral (Integer 42); VLiteral (Integer 54)] 
-             [VLiteral (Integer 42); VLiteral (Integer 42)]), []|.
+  |inl (VMap [VLit (Integer 42); VLit (Integer 54)] 
+             [VLit (Integer 42); VLit (Integer 42)]), []|.
 Proof.
-  eapply eval_map with (kvals := [VLiteral (Integer 54); VLiteral (Integer 42)])
-                       (vvals := [VLiteral (Integer 42); VLiteral (Integer 42)])
+  eapply eval_map with (kvals := [VLit (Integer 54); VLit (Integer 42)])
+                       (vvals := [VLit (Integer 42); VLit (Integer 42)])
                        (eff := [[];[];[];[]]); auto.
   * intros. inversion H.
     - apply eval_var.
@@ -624,15 +624,15 @@ Proof.
 Qed.
 
 Example map_eval3 : 
-  |[(inl "X"%string, VLiteral (Integer 5))], 
-   EMap [ELiteral (Integer 5); EVar "X"%string] 
+  |[(inl "X"%string, VLit (Integer 5))], 
+   EMap [ELit (Integer 5); EVar "X"%string] 
         [EVar "X"%string; ECall "plus" 
-                              [ELiteral (Integer 1); (EVar "X"%string)]], []| 
+                              [ELit (Integer 1); (EVar "X"%string)]], []| 
 -e> 
-  |inl (VMap [VLiteral (Integer 5)] [VLiteral (Integer 6)]), []|.
+  |inl (VMap [VLit (Integer 5)] [VLit (Integer 6)]), []|.
 Proof.
-  apply eval_map with (kvals := [VLiteral (Integer 5); VLiteral (Integer 5)])
-                      (vvals := [VLiteral (Integer 5); VLiteral (Integer 6)])
+  apply eval_map with (kvals := [VLit (Integer 5); VLit (Integer 5)])
+                      (vvals := [VLit (Integer 5); VLit (Integer 6)])
                       (eff := [[];[];[];[]]); auto.
   * intros. inversion H.
     - apply eval_var.
@@ -640,7 +640,7 @@ Proof.
       + apply eval_lit.
       + inversion H3.
   * intros. inversion H.
-    - eapply eval_call with (vals := [VLiteral (Integer 1); VLiteral (Integer 5)])
+    - eapply eval_call with (vals := [VLit (Integer 1); VLit (Integer 5)])
                             (eff := [[];[]]); auto.
       + intros. inversion H0.
         ** apply eval_var.
@@ -655,34 +655,34 @@ Qed.
 (** Function parameter always overwrites everything *)
 Example let_closure_apply_eval_without_overwrite :
   |[], 
-   ELet ["X"%string] [ELiteral (Integer 42)] 
+   ELet ["X"%string] [ELit (Integer 42)] 
      (ELet ["Y"%string] [EFun ["X"%string] (EVar "X"%string)] 
-       (ELet ["X"%string] [ELiteral (Integer 5)] 
-         (EApply (EVar "Y"%string) [ELiteral (Integer 7)]))), []|
+       (ELet ["X"%string] [ELit (Integer 5)] 
+         (EApp (EVar "Y"%string) [ELit (Integer 7)]))), []|
 -e>
-  |inl (VLiteral (Integer 7)), []|.
+  |inl (VLit (Integer 7)), []|.
 Proof.
-  eapply eval_let with (vals := [VLiteral (Integer 42)]) (eff := [[]]); auto.
+  eapply eval_let with (vals := [VLit (Integer 42)]) (eff := [[]]); auto.
   * simpl. intros. inversion H.
     - apply eval_lit.
     - inversion H1.
   * reflexivity.
   * simpl. eapply eval_let with 
-             (vals := [VClosure [(inl "X"%string, VLiteral (Integer 42))] [] 
+             (vals := [VClos [(inl "X"%string, VLit (Integer 42))] [] 
                           0 ["X"%string] (EVar "X"%string)])
              (eff := [[]]); auto.
     - simpl. intros. inversion H.
       + apply eval_fun.
       + inversion H1.
     - reflexivity.
-    - simpl. eapply eval_let with (vals := [VLiteral (Integer 5)]) (eff := [[]]); auto.
+    - simpl. eapply eval_let with (vals := [VLit (Integer 5)]) (eff := [[]]); auto.
       + simpl. intros. inversion H.
         ** apply eval_lit.
         ** inversion H1.
       + reflexivity.
       + simpl. eapply eval_apply with 
-                    (vals := [VLiteral (Integer 7)]) (n := 0)
-                    (ref := [(inl "X"%string, VLiteral (Integer 42))]) 
+                    (vals := [VLit (Integer 7)]) (n := 0)
+                    (ref := [(inl "X"%string, VLit (Integer 42))]) 
                     (ext := []) (body := (EVar "X"%string)) 
                     (var_list := ["X"%string]) (eff := [[]]); auto.
         ** simpl. intros. apply eval_var.
@@ -697,30 +697,30 @@ Qed.
 (** Example to test that value overwriting does not affect the value in the closure *)
 Example let_closure_apply_eval_without_overwrite2 :
   |[],
-   ELet ["X"%string] [ELiteral (Integer 42)] 
+   ELet ["X"%string] [ELit (Integer 42)] 
      (ELet ["Y"%string] [EFun [] (EVar "X"%string)] 
-       (ELet ["X"%string] [ELiteral (Integer 5)] 
-         (EApply (EVar "Y"%string) []))), []|
+       (ELet ["X"%string] [ELit (Integer 5)] 
+         (EApp (EVar "Y"%string) []))), []|
 -e> 
-  |inl (VLiteral (Integer 42)), []|.
+  |inl (VLit (Integer 42)), []|.
 Proof.
-  eapply eval_let with (vals := [VLiteral (Integer 42)]) (eff := [[]]); auto.
+  eapply eval_let with (vals := [VLit (Integer 42)]) (eff := [[]]); auto.
   * intros. inversion H; inversion H1.
     - apply eval_lit.
   * reflexivity.
   * simpl. eapply eval_let with 
-               (vals := [VClosure [(inl "X"%string, VLiteral (Integer 42))] []
+               (vals := [VClos [(inl "X"%string, VLit (Integer 42))] []
                             0 [] (EVar "X"%string)]) (eff := [[]]); auto.
     - intros. inversion H; inversion H1.
       + apply eval_fun.
     - reflexivity.
-    - eapply eval_let with (vals := [VLiteral (Integer 5)]) (eff := [[]]); auto.
+    - eapply eval_let with (vals := [VLit (Integer 5)]) (eff := [[]]); auto.
       + intros. inversion H; inversion H1.
         ** apply eval_lit.
       + reflexivity.
       + simpl. eapply eval_apply with (vals := []) (var_list := []) 
                                       (body := (EVar "X"%string)) (n := 0)
-                                      (ref := [(inl "X"%string, VLiteral (Integer 42))]) 
+                                      (ref := [(inl "X"%string, VLit (Integer 42))]) 
                                       (ext := []) (eff := []); auto.
         ** apply eval_var.
         ** intros. inversion H.
@@ -729,12 +729,12 @@ Proof.
 Qed.
 
 Example call_eval : 
-  |[(inl "X"%string, VLiteral (Integer 5))], 
-   ECall "plus"%string [EVar "X"%string ; ELiteral (Integer 2)], []|
+  |[(inl "X"%string, VLit (Integer 5))], 
+   ECall "plus"%string [EVar "X"%string ; ELit (Integer 2)], []|
 -e> 
-  |inl (VLiteral (Integer 7)), []|.
+  |inl (VLit (Integer 7)), []|.
 Proof.
-  eapply eval_call with (vals := ([VLiteral (Integer 5) ; VLiteral (Integer 2)]))
+  eapply eval_call with (vals := ([VLit (Integer 5) ; VLit (Integer 2)]))
                         (eff := [[];[]]); auto.
   * simpl. intros. inversion H.
     - apply eval_lit.
@@ -745,16 +745,16 @@ Qed.
 
 Example mutliple_function_let : 
   |[], 
-   ELet ["Z"%string] [ECall "plus"%string [ELiteral (Integer 2) ; ELiteral (Integer 2)] ] 
+   ELet ["Z"%string] [ECall "plus"%string [ELit (Integer 2) ; ELit (Integer 2)] ] 
      (ELet ["Y"%string] [EFun [] (EVar "Z"%string)] 
-        (ELet ["X"%string] [EFun [] (EApply (EVar "Y"%string) [])] 
-          (EApply (EVar "X"%string) []))), []|
+        (ELet ["X"%string] [EFun [] (EApp (EVar "Y"%string) [])] 
+          (EApp (EVar "X"%string) []))), []|
 -e>
-  | inl (VLiteral (Integer 4)), []|.
+  | inl (VLit (Integer 4)), []|.
 Proof.
-  eapply eval_let with (vals := [VLiteral (Integer 4)]) (eff := [[]]); auto.
+  eapply eval_let with (vals := [VLit (Integer 4)]) (eff := [[]]); auto.
   * simpl. intros. inversion H.
-    - eapply eval_call with (vals := [VLiteral (Integer 2); VLiteral (Integer 2)])
+    - eapply eval_call with (vals := [VLit (Integer 2); VLit (Integer 2)])
                             (eff := [[];[]]); auto.
       + simpl. intros. inversion H0.
         ** apply eval_lit.
@@ -763,7 +763,7 @@ Proof.
           -- inversion H5.
     - inversion H1.
   * reflexivity.
-  * simpl. eapply eval_let with (vals := [VClosure [(inl "Z"%string, VLiteral (Integer 4))] [] 
+  * simpl. eapply eval_let with (vals := [VClos [(inl "Z"%string, VLit (Integer 4))] [] 
                                              0 [] (EVar "Z"%string)])
                                 (eff := [[]]); auto.
     - simpl. intros. inversion H.
@@ -771,20 +771,20 @@ Proof.
       + inversion H1.
     - reflexivity.
     - simpl. eapply eval_let with 
-              (vals := [VClosure [(inl "Z"%string, VLiteral (Integer 4));
+              (vals := [VClos [(inl "Z"%string, VLit (Integer 4));
                                     (inl "Y"%string,
-                                    VClosure [(inl "Z"%string, VLiteral (Integer 4))] [] 0 []
-                                      (EVar "Z"%string))] [] 1 [] (EApply (EVar "Y"%string) [])])
+                                    VClos [(inl "Z"%string, VLit (Integer 4))] [] 0 []
+                                      (EVar "Z"%string))] [] 1 [] (EApp (EVar "Y"%string) [])])
               (eff := [[]]); auto.
       + simpl. intros. inversion H.
         ** apply eval_fun.
         ** inversion H1.
       + reflexivity.
       + simpl. eapply eval_apply with (vals := []) (var_list := []) 
-                                      (body := (EApply (EVar "Y"%string) [])) 
-                                      (ref := [(inl "Z"%string, VLiteral (Integer 4));
+                                      (body := (EApp (EVar "Y"%string) [])) 
+                                      (ref := [(inl "Z"%string, VLit (Integer 4));
                                                (inl "Y"%string,
-                                                VClosure [(inl "Z"%string, VLiteral (Integer 4))] 
+                                                VClos [(inl "Z"%string, VLit (Integer 4))] 
                                                        [] 0 [] (EVar "Z"%string))])
                                       (ext := []) (n := 1)
                                       (eff := []); auto.
@@ -793,7 +793,7 @@ Proof.
         ** reflexivity.
         ** simpl. eapply eval_apply with (vals := []) (var_list := []) 
                                          (body := (EVar "Z"%string)) (n := 0)
-                                         (ref := [(inl "Z"%string, VLiteral (Integer 4))]) 
+                                         (ref := [(inl "Z"%string, VLit (Integer 4))]) 
                                          (ext := []) (eff := []); auto.
           -- apply eval_var.
           -- intros. inversion H.
@@ -804,9 +804,9 @@ Qed.
 Example case_eval : 
   |[(inl "X"%string, VEmptyTuple)],
    ECase (EVar "X"%string)
-         [(PLiteral (Integer 5)); (PLiteral (Integer 6)); (PVar "Z"%string) ]
-         [(ELiteral (Atom "true"%string)); (ELiteral (Atom "true"%string)); (ELiteral (Atom "true"%string))]
-         [(ELiteral (Integer 5)); (ELiteral (Integer 6)); (EVar "Z"%string)], []| 
+         [(PLit (Integer 5)); (PLit (Integer 6)); (PVar "Z"%string) ]
+         [(ELit (Atom "true"%string)); (ELit (Atom "true"%string)); (ELit (Atom "true"%string))]
+         [(ELit (Integer 5)); (ELit (Integer 6)); (EVar "Z"%string)], []| 
 -e> 
   |inl (VEmptyTuple), []|.
 Proof.
@@ -826,10 +826,10 @@ Qed.
 Example case_eval2 :
   |[(inl "X"%string, VEmptyTuple)],
    ECase (EVar "X"%string) 
-         [(PLiteral (Integer 5)); (PLiteral (Integer 6)); (PVar "Z"%string); (PVar "Z"%string)]
-         [(ELiteral (Atom "true"%string)); (ELiteral (Atom "true"%string)); 
-          (ELiteral (Atom "false"%string)); (ELiteral (Atom "true"%string))]
-         [(ELiteral (Integer 5)); (ELiteral (Integer 6)); (EVar "Z"%string); (EEmptyMap)], []|
+         [(PLit (Integer 5)); (PLit (Integer 6)); (PVar "Z"%string); (PVar "Z"%string)]
+         [(ELit (Atom "true"%string)); (ELit (Atom "true"%string)); 
+          (ELit (Atom "false"%string)); (ELit (Atom "true"%string))]
+         [(ELit (Integer 5)); (ELit (Integer 6)); (EVar "Z"%string); (EEmptyMap)], []|
 -e> 
   |inl (VEmptyMap), []|.
 Proof.
@@ -851,14 +851,14 @@ Proof.
 Qed.
 
 Example case_eval_fun : 
-  |[(inl "X"%string, VClosure [(inl "Y"%string, ttrue)] [] 0 [] (EVar "Y"%string))], 
+  |[(inl "X"%string, VClos [(inl "Y"%string, ttrue)] [] 0 [] (EVar "Y"%string))], 
    ECase (EVar "X"%string) 
-         [(PLiteral (Integer 5)); (PLiteral (Integer 6)); (PVar "Z"%string)] 
-         [(ELiteral (Atom "true"%string)); (ELiteral (Atom "true"%string)); (ELiteral (Atom "true"%string))] 
-         [(ELiteral (Integer 5)); (ELiteral (Integer 6)); (EApply (EVar "Z"%string) [])], []| 
+         [(PLit (Integer 5)); (PLit (Integer 6)); (PVar "Z"%string)] 
+         [(ELit (Atom "true"%string)); (ELit (Atom "true"%string)); (ELit (Atom "true"%string))] 
+         [(ELit (Integer 5)); (ELit (Integer 6)); (EApp (EVar "Z"%string) [])], []| 
 -e> |inl (ttrue), []|.
 Proof.
-  eapply eval_case with (i := 2) (v := VClosure [(inl "Y"%string, ttrue)] [] 0 [] (EVar "Y"%string)); auto.
+  eapply eval_case with (i := 2) (v := VClos [(inl "Y"%string, ttrue)] [] 0 [] (EVar "Y"%string)); auto.
   * apply eval_var.
   * simpl. reflexivity.
   * intros. inversion H.
@@ -880,10 +880,10 @@ Qed.
 
 
 Example letrec_eval : 
-  |[(inr ("fun4"%string, 0), VClosure [] [(("fun4"%string, 0), ([], EEmptyMap))] 0 [] (EEmptyMap)) ; 
-    (inl "X"%string, VLiteral (Integer 42))],
-   ELetrec [("fun2"%string, 0); ("fun4"%string, 1)] [[]; ["Z"%string]] [(EVar "X"%string) ; (EVar "Z"%string)] 
-     (EApply (EFunId ("fun4"%string, 0)) []), []|
+  |[(inr ("fun4"%string, 0), VClos [] [(("fun4"%string, 0), ([], EEmptyMap))] 0 [] (EEmptyMap)) ; 
+    (inl "X"%string, VLit (Integer 42))],
+   ELetRec [("fun2"%string, 0); ("fun4"%string, 1)] [[]; ["Z"%string]] [(EVar "X"%string) ; (EVar "Z"%string)] 
+     (EApp (EFunId ("fun4"%string, 0)) []), []|
 -e>
   |inl (VEmptyMap), []|.
 Proof.
@@ -901,15 +901,15 @@ Qed.
 
 
 Example unnamed_eval : 
-  |[(inl "X"%string, VLiteral (Integer 5))], 
-   EApply (EFun ["Y"%string] (EVar "Y"%string)) [EVar "X"%string], []|
+  |[(inl "X"%string, VLit (Integer 5))], 
+   EApp (EFun ["Y"%string] (EVar "Y"%string)) [EVar "X"%string], []|
 -e> 
-  |inl (VLiteral (Integer 5)), []|.
+  |inl (VLit (Integer 5)), []|.
 Proof.
-  eapply eval_apply with (vals := [VLiteral (Integer 5)]) 
+  eapply eval_apply with (vals := [VLit (Integer 5)]) 
                          (var_list := ["Y"%string]) 
                          (body := (EVar "Y"%string)) 
-                         (ref := [(inl "X"%string, VLiteral (Integer 5))]) 
+                         (ref := [(inl "X"%string, VLit (Integer 5))]) 
                          (ext := []) (eff := [[]]); auto.
   * apply eval_fun.
   * intros. inversion H; inversion H1. apply eval_var.
@@ -921,37 +921,37 @@ Qed.
 Section B_Core.
 
 Definition B : ErlModule := ErlMod "b"%string [
-  TopLevelFun ("fun1"%string, 0) ([], (ELiteral (Integer 6))) ;
-  TopLevelFun ("fun2"%string, 0) ([], (ELet ["X"%string] [(EFun [] (ELiteral (Integer 5)))] (
-                                         ELet ["X"%string] [(EFun [] (ELiteral (Integer 6)))] 
-                                           (EApply (EVar "X"%string) []))) )
+  TopLevelFun ("fun1"%string, 0) ([], (ELit (Integer 6))) ;
+  TopLevelFun ("fun2"%string, 0) ([], (ELet ["X"%string] [(EFun [] (ELit (Integer 5)))] (
+                                         ELet ["X"%string] [(EFun [] (ELit (Integer 6)))] 
+                                           (EApp (EVar "X"%string) []))) )
 ].
 
 
 Example fun2 : 
   |[], 
-   ELet ["X"%string] [(EFun [] (ELiteral (Integer 5)))] 
-     (ELet ["X"%string] [(EFun [] (ELiteral (Integer 6)))] 
-       (EApply (EVar "X"%string) [])), []|
+   ELet ["X"%string] [(EFun [] (ELit (Integer 5)))] 
+     (ELet ["X"%string] [(EFun [] (ELit (Integer 6)))] 
+       (EApp (EVar "X"%string) [])), []|
 -e>
-  | inl (VLiteral (Integer 6)), []|.
+  | inl (VLit (Integer 6)), []|.
 Proof.
-  eapply eval_let with (vals := [VClosure [] [] 0 [] (ELiteral (Integer 5))]) (eff := [[]]); auto.
+  eapply eval_let with (vals := [VClos [] [] 0 [] (ELit (Integer 5))]) (eff := [[]]); auto.
   * simpl. intros. inversion H.
     - apply eval_fun.
     - inversion H1.
   * reflexivity.
-  * simpl. eapply eval_let with (vals := [VClosure [(inl "X"%string, 
-                                             VClosure [] [] 0 [] (ELiteral (Integer 5)))] 
-                                           [] 1 [] (ELiteral (Integer 6))])
+  * simpl. eapply eval_let with (vals := [VClos [(inl "X"%string, 
+                                             VClos [] [] 0 [] (ELit (Integer 5)))] 
+                                           [] 1 [] (ELit (Integer 6))])
                                 (eff := [[]]); auto.
     - simpl. intros. inversion H.
       + apply eval_fun.
       + inversion H1.
     - reflexivity.
     - simpl. eapply eval_apply with (vals := []) (var_list := []) 
-                                    (body := (ELiteral (Integer 6))) 
-                                    (ref := [(inl "X"%string, VClosure [] [] 0 [] (ELiteral (Integer 5)))]) (n := 1)
+                                    (body := (ELit (Integer 6))) 
+                                    (ref := [(inl "X"%string, VClos [] [] 0 [] (ELit (Integer 5)))]) (n := 1)
                                     (ext := []) (eff := []); auto.
       + apply eval_var.
       + intros. inversion H.
@@ -968,11 +968,11 @@ End B_Core.
 Section Documentation_Examples.
 
 Example ex1 : 
-  |[], ELet ["X"%string] [ELiteral (Integer 5)] (EVar "X"%string), []|
+  |[], ELet ["X"%string] [ELit (Integer 5)] (EVar "X"%string), []|
 -e>
-  |inl (VLiteral (Integer 5)), []|.
+  |inl (VLit (Integer 5)), []|.
 Proof.
-  eapply eval_let with (vals := [VLiteral (Integer 5)]) (eff := [[]]).
+  eapply eval_let with (vals := [VLit (Integer 5)]) (eff := [[]]).
   * reflexivity.
   * reflexivity.
   * intros. inversion H.
@@ -984,19 +984,19 @@ Qed.
 
 Example ex2 : 
   |[],
-   ELet ["X"%string] [EFun [] (EApply (EVar "X"%string) [])] 
-     (EApply (EVar "X"%string) []), []|
+   ELet ["X"%string] [EFun [] (EApp (EVar "X"%string) [])] 
+     (EApp (EVar "X"%string) []), []|
 -e>
   |inr novar, []|.
 Proof.
-  eapply eval_let with (vals := [VClosure [] [] 0 [] (EApply ( EVar "X"%string) [])])
+  eapply eval_let with (vals := [VClos [] [] 0 [] (EApp ( EVar "X"%string) [])])
                        (eff := [[]]); auto.
   * intros. inversion H.
     - subst. apply eval_fun.
     - inversion H1.
   * reflexivity.
   * simpl. eapply eval_apply with (vals := []) (var_list := []) 
-                                  (body := (EApply (EVar "X"%string) [])) 
+                                  (body := (EApp (EVar "X"%string) [])) 
                                   (ref := []) (ext := []) (n := 0) (eff := []); auto.
     - apply eval_var.
     - intros. inversion H.
@@ -1007,30 +1007,30 @@ Proof.
 Qed.
 
 Example ex3 :
-  |[], ELetrec [("X"%string, 0)] [[]] [(EApply (EFunId ("X"%string, 0)) [])] 
-         (EApply (EFunId ("X"%string, 0)) []), []|
+  |[], ELetRec [("X"%string, 0)] [[]] [(EApp (EFunId ("X"%string, 0)) [])] 
+         (EApp (EFunId ("X"%string, 0)) []), []|
 -e>
   |inl (VEmptyTuple), []|.
 Proof.
   eapply eval_letrec; try (reflexivity).
   * simpl. eapply eval_apply with (vals := []) (var_list := []) (ref := []) (n := 0) (eff := [])
-                                  (body := (EApply (EFunId ("X"%string, 0)) []))
-                                  (ext := [("X"%string, 0, ([], EApply (EFunId ("X"%string, 0)) []))]); 
+                                  (body := (EApp (EFunId ("X"%string, 0)) []))
+                                  (ext := [("X"%string, 0, ([], EApp (EFunId ("X"%string, 0)) []))]); 
         try (reflexivity).
     - apply eval_funid.
     - intros. inversion H.
     - reflexivity.
     - simpl. eapply eval_apply with (vals := []) (n := 0) (var_list := []) (ref := []) (eff := [])
-                                    (body := (EApply (EFunId ("X"%string, 0)) []))
-                                    (ext := [("X"%string, 0, ([], EApply (EFunId ("X"%string, 0)) []))]); 
+                                    (body := (EApp (EFunId ("X"%string, 0)) []))
+                                    (ext := [("X"%string, 0, ([], EApp (EFunId ("X"%string, 0)) []))]); 
          try (reflexivity).
       + apply eval_funid.
       + intros. inversion H.
       + reflexivity.
       + simpl. eapply eval_apply with (vals := []) (var_list := []) (n := 0) (ref := []) (eff := [])
-                                      (body := (EApply (EFunId ("X"%string, 0)) [])) 
+                                      (body := (EApp (EFunId ("X"%string, 0)) [])) 
                                       (ext := [("X"%string, 0, 
-                                               ([], EApply (EFunId ("X"%string, 0)) []))]); 
+                                               ([], EApp (EFunId ("X"%string, 0)) []))]); 
              try (reflexivity).
         ** apply eval_funid.
         ** intros. inversion H.
@@ -1038,31 +1038,31 @@ Proof.
 Admitted.
 
 Example ex4 : 
-|[], ELet ["X"%string] [ELiteral (Integer 4)] 
+|[], ELet ["X"%string] [ELit (Integer 4)] 
        (ELet ["X"%string] [EFun [] (EVar "X"%string)] 
-          (ELet ["X"%string] [EFun [] (EApply (EVar "X"%string) [])] 
-             (EApply (EVar "X"%string) []))), []|
+          (ELet ["X"%string] [EFun [] (EApp (EVar "X"%string) [])] 
+             (EApp (EVar "X"%string) []))), []|
 -e>
-  |inl (VLiteral (Integer 4)), []|.
+  |inl (VLit (Integer 4)), []|.
 Proof.
-  eapply eval_let with (vals := [VLiteral (Integer 4)]) (eff := [[]]); auto.
+  eapply eval_let with (vals := [VLit (Integer 4)]) (eff := [[]]); auto.
   * intros. inversion H; inversion H1. apply eval_lit.
   * reflexivity.
-  * simpl. eapply eval_let with (vals := [VClosure [(inl "X"%string, VLiteral (Integer 4))] [] 0 [] 
+  * simpl. eapply eval_let with (vals := [VClos [(inl "X"%string, VLit (Integer 4))] [] 0 [] 
                                             (EVar "X"%string)])
                                 (eff := [[]]); auto.
     - intros. inversion H; inversion H1. apply eval_fun.
     - reflexivity.
-    - simpl. eapply eval_let with (vals := [VClosure [(inl "X"%string,
-                                              VClosure [(inl "X"%string, VLiteral (Integer 4))] [] 0 []
-                                                (EVar "X"%string))] [] 1 [] (EApply (EVar "X"%string) []) ])
+    - simpl. eapply eval_let with (vals := [VClos [(inl "X"%string,
+                                              VClos [(inl "X"%string, VLit (Integer 4))] [] 0 []
+                                                (EVar "X"%string))] [] 1 [] (EApp (EVar "X"%string) []) ])
                                   (eff := [[]]); auto.
        + intros. inversion H; inversion H1. apply eval_fun.
        + reflexivity.
        + simpl. eapply eval_apply with (vals := []) (var_list := []) 
-                                       (body := EApply (EVar "X"%string) []) 
+                                       (body := EApp (EVar "X"%string) []) 
                                        (ref := [(inl "X"%string,
-                                                 VClosure [(inl "X"%string, VLiteral (Integer 4))] [] 0 []
+                                                 VClos [(inl "X"%string, VLit (Integer 4))] [] 0 []
                                                    (EVar "X"%string))]) (n := 1)
                                        (ext := []) (eff := []); auto.
          ** apply eval_var.
@@ -1070,7 +1070,7 @@ Proof.
          ** reflexivity.
          ** simpl. eapply eval_apply with (vals := []) (var_list := []) 
                                           (body := EVar "X"%string) 
-                                          (ref := [(inl "X"%string, VLiteral (Integer 4))]) (n := 0)
+                                          (ref := [(inl "X"%string, VLit (Integer 4))]) (n := 0)
                                           (ext := []) (eff := []); auto.
            -- apply eval_var.
            -- intros. inversion H.
@@ -1082,19 +1082,19 @@ End Documentation_Examples.
 
 Example returned_function :
   |[], 
-   ELet ["X"%string] [EFun [] (EFun [] (ELiteral (Integer 5)))] 
-     (EApply (EApply (EVar "X"%string) []) []), []|
+   ELet ["X"%string] [EFun [] (EFun [] (ELit (Integer 5)))] 
+     (EApp (EApp (EVar "X"%string) []) []), []|
 -e>
-  |inl (VLiteral (Integer 5)), []|.
+  |inl (VLit (Integer 5)), []|.
 Proof.
-  eapply eval_let with (vals := [VClosure [] [] 0 [] (EFun [] (ELiteral (Integer 5)))])
+  eapply eval_let with (vals := [VClos [] [] 0 [] (EFun [] (ELit (Integer 5)))])
                        (eff := [[]]); auto.
   * intros. inversion H; inversion H1. apply eval_fun.
   * reflexivity.
   * simpl. eapply eval_apply with (vals := []) (ref := []) (ext := []) (eff := [])
-                                  (body := ELiteral (Integer 5)) (var_list := []); auto.
+                                  (body := ELit (Integer 5)) (var_list := []); auto.
     - eapply eval_apply with (vals := []) (var_list := []) (n := 0)
-                             (body := EFun [] (ELiteral (Integer 5))) 
+                             (body := EFun [] (ELit (Integer 5))) 
                              (ref := []) (ext := []) (eff := []); auto.
       + apply eval_var.
       + intros. inversion H.
@@ -1107,22 +1107,22 @@ Qed.
 
 Example returned_recursive_function : 
   |[], 
-   ELetrec [("fun1"%string, 0)] [[]] [(EFun [] (ELiteral (Integer 5)))] 
-     (EApply (EApply (EFunId ("fun1"%string, 0)) []) []), []|
+   ELetRec [("fun1"%string, 0)] [[]] [(EFun [] (ELit (Integer 5)))] 
+     (EApp (EApp (EFunId ("fun1"%string, 0)) []) []), []|
 -e>
-  |inl (VLiteral (Integer 5)), []|.
+  |inl (VLit (Integer 5)), []|.
 Proof.
   eapply eval_letrec; try (reflexivity).
   * simpl. eapply eval_apply with (vals := []) (ref := [(inr ("fun1"%string, 0),
-                                                         VClosure [] [("fun1"%string, 0, ([], 
-                                                            EFun [] (ELiteral (Integer 5))))] 0 []
-                                                            (EFun [] (ELiteral (Integer 5))))]) 
-                                  (ext := []) (body := ELiteral (Integer 5)) 
+                                                         VClos [] [("fun1"%string, 0, ([], 
+                                                            EFun [] (ELit (Integer 5))))] 0 []
+                                                            (EFun [] (ELit (Integer 5))))]) 
+                                  (ext := []) (body := ELit (Integer 5)) 
                                   (var_list := []) (eff := []); try (reflexivity).
     - eapply eval_apply with (vals := []) (var_list := []) 
-                             (body := EFun [] (ELiteral (Integer 5))) 
+                             (body := EFun [] (ELit (Integer 5))) 
                              (ref := []) (eff := []) (n := 0)
-                             (ext := [("fun1"%string, 0, ([], EFun [] (ELiteral (Integer 5))))]);
+                             (ext := [("fun1"%string, 0, ([], EFun [] (ELit (Integer 5))))]);
           try (reflexivity).
       + apply eval_funid.
       + intros. inversion H.
@@ -1133,22 +1133,22 @@ Proof.
 Qed.
 
 Example returned_function2 :
-  |[(inl "X"%string, VLiteral (Integer 7))],
+  |[(inl "X"%string, VLit (Integer 7))],
    ELet ["X"%string] [EFun [] (EFun [] (EVar "X"%string))] 
-     (EApply (EApply (EVar "X"%string) []) []), []|
+     (EApp (EApp (EVar "X"%string) []) []), []|
 -e>
-  |inl (VLiteral (Integer 7)), []|.
+  |inl (VLit (Integer 7)), []|.
 Proof.
-  eapply eval_let with (vals := [VClosure [(inl "X"%string, VLiteral (Integer 7))] [] 
+  eapply eval_let with (vals := [VClos [(inl "X"%string, VLit (Integer 7))] [] 
                                   0 [] (EFun [] (EVar "X"%string))])
                        (eff := [[]]); auto.
   * intros. inversion H; inversion H1. apply eval_fun.
   * reflexivity.
-  * simpl. eapply eval_apply with (vals := []) (ref := [(inl "X"%string, VLiteral (Integer 7))]) 
+  * simpl. eapply eval_apply with (vals := []) (ref := [(inl "X"%string, VLit (Integer 7))]) 
                                  (ext := []) (body := EVar "X"%string) (var_list := []) (eff := []) (n := 0); auto.
     - eapply eval_apply with (vals := []) (var_list := []) 
                              (body := EFun [] (EVar "X"%string)) 
-                             (ref := [(inl "X"%string, VLiteral (Integer 7))]) 
+                             (ref := [(inl "X"%string, VLit (Integer 7))]) 
                              (ext := []) (n := 0) (eff := []); auto.
       + apply eval_var.
       + intros. inversion H.
@@ -1160,17 +1160,17 @@ Proof.
 Qed.
 
 Example returned_recursive_function2 :
-  |[(inl "X"%string, VLiteral (Integer 7))], 
-   ELetrec [("fun1"%string, 0)] [[]] [(EFun [] (EVar "X"%string))] 
-     (EApply (EApply (EFunId ("fun1"%string, 0)) []) []), []|
+  |[(inl "X"%string, VLit (Integer 7))], 
+   ELetRec [("fun1"%string, 0)] [[]] [(EFun [] (EVar "X"%string))] 
+     (EApp (EApp (EFunId ("fun1"%string, 0)) []) []), []|
 -e>
-  |inl (VLiteral (Integer 7)), []|.
+  |inl (VLit (Integer 7)), []|.
 Proof.
   eapply eval_letrec; try (reflexivity).
   * simpl. eapply eval_apply with (vals := []) (eff := [])
-                                 (ref := [(inl "X"%string, VLiteral (Integer 7)) ; 
+                                 (ref := [(inl "X"%string, VLit (Integer 7)) ; 
                                           (inr ("fun1"%string, 0),
-                                             VClosure [(inl "X"%string, VLiteral (Integer 7))] 
+                                             VClos [(inl "X"%string, VLit (Integer 7))] 
                                                       [("fun1"%string, 0, 
                                                           ([], EFun [] (EVar "X"%string)))] 
                                                       0 [] 
@@ -1179,7 +1179,7 @@ Proof.
                                  (var_list := []) (ext := []); try (reflexivity).
     - eapply eval_apply with (vals := []) (var_list := []) (eff := [])
                              (body := EFun [] (EVar "X"%string)) (n := 0)
-                             (ref := [(inl "X"%string, VLiteral (Integer 7))]) 
+                             (ref := [(inl "X"%string, VLit (Integer 7))]) 
                              (ext := [("fun1"%string, 0, ([], EFun [] (EVar "X"%string)))]); 
           try (reflexivity).
       + apply eval_funid.
@@ -1195,18 +1195,18 @@ Example returned_function3 :
    ELet ["F"%string] [
      EFun ["X"%string] 
         (ELet ["Y"%string] 
-              [ECall "plus"%string [EVar "X"%string; ELiteral (Integer 3)] ] 
+              [ECall "plus"%string [EVar "X"%string; ELit (Integer 3)] ] 
               (EFun ["Z"%string] 
                     (ECall "plus"%string 
                           [ECall "plus"%string [EVar "X"%string; EVar "Y"%string]
                      ; EVar "Z"%string])))]
-  (EApply (EApply (EVar "F"%string) [ELiteral (Integer 1)]) [ELiteral (Integer 1)]), []|
+  (EApp (EApp (EVar "F"%string) [ELit (Integer 1)]) [ELit (Integer 1)]), []|
 -e>
-  |inl (VLiteral (Integer 6)), []|.
+  |inl (VLit (Integer 6)), []|.
 Proof.
-  eapply eval_let with (vals := [VClosure [] [] 0 ["X"%string] (ELet ["Y"%string]
+  eapply eval_let with (vals := [VClos [] [] 0 ["X"%string] (ELet ["Y"%string]
                                         [ECall "plus"
-                                           [EVar "X"%string; ELiteral (Integer 3)] ]
+                                           [EVar "X"%string; ELit (Integer 3)] ]
                                         (EFun ["Z"%string]
                                            (ECall "plus"
                                               [ECall "plus"
@@ -1220,13 +1220,13 @@ Proof.
                                               [ECall "plus"
                                                  [EVar "X"%string; EVar "Y"%string];
                                               EVar "Z"%string]))
-                                  (ref := [(inl "X"%string, VLiteral (Integer 1)); 
-                                           (inl "Y"%string, VLiteral (Integer 4))])
-                                  (ext := []) (vals := [VLiteral (Integer 1)]); auto.
-    - eapply eval_apply with (vals := [VLiteral (Integer 1)]) (var_list := ["X"%string]) 
+                                  (ref := [(inl "X"%string, VLit (Integer 1)); 
+                                           (inl "Y"%string, VLit (Integer 4))])
+                                  (ext := []) (vals := [VLit (Integer 1)]); auto.
+    - eapply eval_apply with (vals := [VLit (Integer 1)]) (var_list := ["X"%string]) 
                              (body := ELet ["Y"%string]
                                         [ECall "plus"
-                                           [EVar "X"%string; ELiteral (Integer 3)] ]
+                                           [EVar "X"%string; ELit (Integer 3)] ]
                                         (EFun ["Z"%string]
                                            (ECall "plus"
                                               [ECall "plus"
@@ -1236,9 +1236,9 @@ Proof.
       + apply eval_var.
       + intros. inversion H; inversion H1. apply eval_lit.
       + reflexivity.
-      + eapply eval_let with (vals := [VLiteral (Integer 4)]) (eff := [[]]); auto.
+      + eapply eval_let with (vals := [VLit (Integer 4)]) (eff := [[]]); auto.
         ** intros. inversion H; inversion H1. 
-           apply eval_call with (vals := [VLiteral (Integer 1); VLiteral (Integer 3)])
+           apply eval_call with (vals := [VLit (Integer 1); VLit (Integer 3)])
                                 (eff := [[];[]]); auto.
           -- intros. inversion H2.
             ++ apply eval_lit.
@@ -1246,12 +1246,12 @@ Proof.
         ** simpl. apply eval_fun.
     - intros. inversion H; inversion H1. apply eval_lit.
     - reflexivity.
-    - eapply eval_call with (vals := [VLiteral (Integer 5) ; VLiteral (Integer 1)])
+    - eapply eval_call with (vals := [VLit (Integer 5) ; VLit (Integer 1)])
                             (eff := [[];[]]); auto.
       + intros. inversion H.
         ** inversion H1. apply eval_var.
         ** inversion H1.
-          -- eapply eval_call with (vals := [VLiteral (Integer 1) ; VLiteral (Integer 4)])
+          -- eapply eval_call with (vals := [VLit (Integer 1) ; VLit (Integer 4)])
                                                (eff := [[];[]]); auto.
             ++ intros. inversion H2.
               *** apply eval_var.
@@ -1261,112 +1261,112 @@ Qed.
 
 Example sum :
   | [],
-    ELetrec [("f"%string, 1)] [["X"%string]] 
+    ELetRec [("f"%string, 1)] [["X"%string]] 
       [
-      ECase (EVar "X"%string) [PLiteral (Integer 0); PVar "Y"%string]
-                              [ELiteral (Atom "true"%string); ELiteral (Atom "true"%string)]
+      ECase (EVar "X"%string) [PLit (Integer 0); PVar "Y"%string]
+                              [ELit (Atom "true"%string); ELit (Atom "true"%string)]
                               [
-                              ELiteral (Integer 0)
+                              ELit (Integer 0)
                               ;
                               ECall "plus"%string [
                                      EVar "Y"%string; 
-                                     EApply (EFunId ("f"%string, 1)) [ECall "plus"%string [EVar "Y"%string; ELiteral (Integer (Z.pred 0))] ]
+                                     EApp (EFunId ("f"%string, 1)) [ECall "plus"%string [EVar "Y"%string; ELit (Integer (Z.pred 0))] ]
                               ]
-     ] ] (EApply (EFunId ("f"%string, 1)) [ELiteral (Integer 2)]), []| -e> |inl (VLiteral (Integer 3)), []|.
+     ] ] (EApp (EFunId ("f"%string, 1)) [ELit (Integer 2)]), []| -e> |inl (VLit (Integer 3)), []|.
 Proof.
   eapply eval_letrec; auto.
   2: reflexivity.
-  * simpl. eapply eval_apply with (vals := [VLiteral (Integer 2)]) (eff := [[]]) (eff2 := []) (n := 0)
+  * simpl. eapply eval_apply with (vals := [VLit (Integer 2)]) (eff := [[]]) (eff2 := []) (n := 0)
                                   (var_list := ["X"%string]) (ref := []) 
                                   (body := 
-      (ECase (EVar "X"%string) [PLiteral (Integer 0); PVar "Y"%string]
-        [ELiteral (Atom "true"); ELiteral (Atom "true")]
-        [ELiteral (Integer 0);
+      (ECase (EVar "X"%string) [PLit (Integer 0); PVar "Y"%string]
+        [ELit (Atom "true"); ELit (Atom "true")]
+        [ELit (Integer 0);
         ECall "plus"
           [EVar "Y"%string;
-          EApply (EFunId ("f"%string, 1))
-            [ECall "plus" [EVar "Y"%string; ELiteral (Integer (-1))]]]]))
+          EApp (EFunId ("f"%string, 1))
+            [ECall "plus" [EVar "Y"%string; ELit (Integer (-1))]]]]))
                                   (ext := [("f"%string, 1,
                                       (["X"%string],
-                                      ECase (EVar "X"%string) [PLiteral (Integer 0); PVar "Y"%string]
-                                        [ELiteral (Atom "true"); ELiteral (Atom "true")]
-                                        [ELiteral (Integer 0);
+                                      ECase (EVar "X"%string) [PLit (Integer 0); PVar "Y"%string]
+                                        [ELit (Atom "true"); ELit (Atom "true")]
+                                        [ELit (Integer 0);
                                         ECall "plus"
                                           [EVar "Y"%string;
-                                          EApply (EFunId ("f"%string, 1))
+                                          EApp (EFunId ("f"%string, 1))
                                             [ECall "plus" [EVar "Y"%string; 
-                                                ELiteral (Integer (-1))]]]]))]); simpl; auto.
+                                                ELit (Integer (-1))]]]]))]); simpl; auto.
     - apply eval_funid.
     - intros. inversion H; inversion H1. apply eval_lit.
-    - unfold concatn. simpl. eapply eval_case with (i := 1) (v := VLiteral (Integer 2)); auto.
+    - unfold concatn. simpl. eapply eval_case with (i := 1) (v := VLit (Integer 2)); auto.
       + apply eval_var.
       + simpl. reflexivity.
       + intros. inversion H; inversion H2. subst. inversion H0.
       + reflexivity.
       + simpl. apply eval_lit.
-      + eapply eval_call with (vals := [VLiteral (Integer 2); VLiteral (Integer 1)]) (eff := [[]; []]); auto.
+      + eapply eval_call with (vals := [VLit (Integer 2); VLit (Integer 1)]) (eff := [[]; []]); auto.
         ** intros. inversion H; inversion H1. 3: inversion H3.
-          -- simpl. eapply eval_apply with (vals := [VLiteral (Integer 1)]) (eff := [[]]) (eff2 := [])
+          -- simpl. eapply eval_apply with (vals := [VLit (Integer 1)]) (eff := [[]]) (eff2 := [])
                                   (var_list := ["X"%string]) (ref := []) 
                                   (body := 
-      (ECase (EVar "X"%string) [PLiteral (Integer 0); PVar "Y"%string]
-        [ELiteral (Atom "true"); ELiteral (Atom "true")]
-        [ELiteral (Integer 0);
+      (ECase (EVar "X"%string) [PLit (Integer 0); PVar "Y"%string]
+        [ELit (Atom "true"); ELit (Atom "true")]
+        [ELit (Integer 0);
         ECall "plus"
           [EVar "Y"%string;
-          EApply (EFunId ("f"%string, 1))
-            [ECall "plus" [EVar "Y"%string; ELiteral (Integer (-1))]]]]))
+          EApp (EFunId ("f"%string, 1))
+            [ECall "plus" [EVar "Y"%string; ELit (Integer (-1))]]]]))
                                   (ext := [("f"%string, 1,
                                       (["X"%string],
-                                      ECase (EVar "X"%string) [PLiteral (Integer 0); PVar "Y"%string]
-                                        [ELiteral (Atom "true"); ELiteral (Atom "true")]
-                                        [ELiteral (Integer 0);
+                                      ECase (EVar "X"%string) [PLit (Integer 0); PVar "Y"%string]
+                                        [ELit (Atom "true"); ELit (Atom "true")]
+                                        [ELit (Integer 0);
                                         ECall "plus"
                                           [EVar "Y"%string;
-                                          EApply (EFunId ("f"%string, 1))
+                                          EApp (EFunId ("f"%string, 1))
                                             [ECall "plus" [EVar "Y"%string; 
-                                                ELiteral (Integer (-1))]]]]))]) (n := 0); simpl; auto.
+                                                ELit (Integer (-1))]]]]))]) (n := 0); simpl; auto.
             ++ apply eval_funid.
-            ++ intros. inversion H2; inversion H4. eapply eval_call with (vals := [VLiteral (Integer 2); VLiteral (Integer (-1))]) (eff := [[];[]]); auto.
+            ++ intros. inversion H2; inversion H4. eapply eval_call with (vals := [VLit (Integer 2); VLit (Integer (-1))]) (eff := [[];[]]); auto.
               *** simpl. intros. inversion H5; inversion H7. 3: inversion H9.
                 --- apply eval_lit.
                 --- apply eval_var.
             ++ {
-            eapply eval_case with (i := 1) (v := VLiteral (Integer 1)); auto.
+            eapply eval_case with (i := 1) (v := VLit (Integer 1)); auto.
               + apply eval_var.
               + simpl. reflexivity.
               + intros. inversion H2; inversion H5. subst. inversion H3.
               + reflexivity.
               + simpl. apply eval_lit.
-              + subst. simpl. eapply eval_call with (vals := [VLiteral (Integer 1); VLiteral (Integer (0))]) (eff := [[];[]]); auto.
+              + subst. simpl. eapply eval_call with (vals := [VLit (Integer 1); VLit (Integer (0))]) (eff := [[];[]]); auto.
                 * simpl. intros. inversion H1; inversion H3. 3: inversion H5. 
-                  - eapply eval_apply with (vals := [VLiteral (Integer 0)]) (eff := [[]]) (eff2 := [])
+                  - eapply eval_apply with (vals := [VLit (Integer 0)]) (eff := [[]]) (eff2 := [])
                                   (var_list := ["X"%string]) (ref := []) (n := 0)
                                   (body := 
-      (ECase (EVar "X"%string) [PLiteral (Integer 0); PVar "Y"%string]
-        [ELiteral (Atom "true"); ELiteral (Atom "true")]
-        [ELiteral (Integer 0);
+      (ECase (EVar "X"%string) [PLit (Integer 0); PVar "Y"%string]
+        [ELit (Atom "true"); ELit (Atom "true")]
+        [ELit (Integer 0);
         ECall "plus"
           [EVar "Y"%string;
-          EApply (EFunId ("f"%string, 1))
-            [ECall "plus" [EVar "Y"%string; ELiteral (Integer (-1))]]]]))
+          EApp (EFunId ("f"%string, 1))
+            [ECall "plus" [EVar "Y"%string; ELit (Integer (-1))]]]]))
                                   (ext := [("f"%string, 1,
                                       (["X"%string],
-                                      ECase (EVar "X"%string) [PLiteral (Integer 0); PVar "Y"%string]
-                                        [ELiteral (Atom "true"); ELiteral (Atom "true")]
-                                        [ELiteral (Integer 0);
+                                      ECase (EVar "X"%string) [PLit (Integer 0); PVar "Y"%string]
+                                        [ELit (Atom "true"); ELit (Atom "true")]
+                                        [ELit (Integer 0);
                                         ECall "plus"
                                           [EVar "Y"%string;
-                                          EApply (EFunId ("f"%string, 1))
+                                          EApp (EFunId ("f"%string, 1))
                                             [ECall "plus" [EVar "Y"%string; 
-                                                ELiteral (Integer (-1))]]]]))]); simpl; auto.
+                                                ELit (Integer (-1))]]]]))]); simpl; auto.
                   ** apply eval_funid.
-                  ** intros. inversion H4. 2: inversion H6. eapply eval_call with (vals := [VLiteral (Integer 1); VLiteral (Integer (-1))]) (eff := [[];[]]); auto.
+                  ** intros. inversion H4. 2: inversion H6. eapply eval_call with (vals := [VLit (Integer 1); VLit (Integer (-1))]) (eff := [[];[]]); auto.
                     -- intros. inversion H5; inversion H8.
                       ++ simpl. apply eval_lit.
                       ++ simpl. apply eval_var.
                       ++ inversion H10.
-                  ** eapply eval_case with (i := 0) (v := VLiteral (Integer 0)); auto.
+                  ** eapply eval_case with (i := 0) (v := VLit (Integer 0)); auto.
                     -- apply eval_var.
                     -- simpl. omega.
                     -- reflexivity.
@@ -1381,25 +1381,25 @@ Qed.
 
 Example letrec_no_replace :
   |[], 
-   ELet ["X"%string] [ELiteral (Integer 42)] 
-     (ELetrec [("f"%string, 0)] [[]] [EVar "X"%string]
-       (ELet ["X"%string] [ELiteral (Integer 5)] 
-         (EApply (EFunId ("f"%string, 0)) []))), []|
+   ELet ["X"%string] [ELit (Integer 42)] 
+     (ELetRec [("f"%string, 0)] [[]] [EVar "X"%string]
+       (ELet ["X"%string] [ELit (Integer 5)] 
+         (EApp (EFunId ("f"%string, 0)) []))), []|
 -e>
-  |inl (VLiteral (Integer 42)), []|.
+  |inl (VLit (Integer 42)), []|.
 Proof.
-  eapply eval_let with (vals := [VLiteral (Integer 42)]) (eff := [[]]); auto.
+  eapply eval_let with (vals := [VLit (Integer 42)]) (eff := [[]]); auto.
   * intros. inversion H; inversion H1.
     - apply eval_lit.
   * reflexivity.
   * simpl. eapply eval_letrec; auto.
     2: reflexivity.
-    - eapply eval_let with (vals := [VLiteral (Integer 5)]) (eff := [[]]); auto.
+    - eapply eval_let with (vals := [VLit (Integer 5)]) (eff := [[]]); auto.
       + intros. inversion H; inversion H1.
         ** apply eval_lit.
       + simpl. eapply eval_apply with (vals := []) (var_list := []) 
                                       (body := (EVar "X"%string)) 
-                                      (ref := [(inl "X"%string, VLiteral (Integer 42))]) 
+                                      (ref := [(inl "X"%string, VLit (Integer 42))]) 
                                       (ext := [("f"%string, 0, ([], EVar "X"%string))]) (eff := []) (n := 0); auto.
         ** apply eval_funid.
         ** intros. inversion H.
